started asn_strtoimax spec

asn_strtoimax_lim.light.c
@@ -1,0 +1,86 @@
+int asn_strtoimax_lim(signed char *str, signed char **end, long long *intp)
+{
+  register int $307;
+  register long long $29;
+  register long long $308;
+  register long long $309;
+  register int $310;
+  register signed char *$343;
+  register signed char *$342;
+  register signed char $341;
+  register signed char *$340;
+  register signed char $339;
+  register signed char $338;
+  $307 = 1;
+  $308 = (~((unsigned long long) 0) >> 1) / 10;
+  $309 = (~((unsigned long long) 0) >> 1) % 10;
+  $343 = *$234;
+  if ($305 >= $343) {
+    return -2;
+  }
+  $341 = *$305;
+  switch (*$305) {
+    case 45:
+      $309 = $309 + 1;
+      $307 = -1;
+    case 43:
+      $305 = $305 + 1;
+      $342 = *$234;
+      if ($305 >= $342) {
+        *$234 = $305;
+        return -1;
+      }
+    
+  }
+  $29 = (long long) 0;
+  for (; 1; $305 = $305 + 1) {
+    $340 = *$234;
+    if (! ($305 < $340)) {
+      break;
+    }
+    $338 = *$305;
+    switch (*$305) {
+      case 48:
+      case 49:
+      case 50:
+      case 51:
+      case 52:
+      case 53:
+      case 54:
+      case 55:
+      case 56:
+      case 57:
+        $339 = *$305;
+        $310 = $339 - 48;
+        if ($29 < $308) {
+          $29 = $29 * 10 + $310;
+        } else {
+          if ($29 == $308) {
+            if ($310 <= $309) {
+              if ($307 > 0) {
+                $29 = $29 * 10 + $310;
+              } else {
+                $307 = 1;
+                $29 = -$29 * 10 - $310;
+              }
+            } else {
+              *$234 = $305;
+              return -3;
+            }
+          } else {
+            *$234 = $305;
+            return -3;
+          }
+        }
+        continue;
+      default:
+        *$234 = $305;
+        *$306 = $307 * $29;
+        return 1;
+      
+    }
+  }
+  *$234 = $305;
+  *$306 = $307 * $29;
+  return 0;
+}
