BOOLEAN.v
@@ -1,0 +1,2669 @@
+From Coq Require Import String List ZArith.
+From compcert Require Import Coqlib Integers Floats AST Ctypes Cop Clight Clightdefs.
+Local Open Scope Z_scope.
+
+Module Info.
+  Definition version := "3.4"%string.
+  Definition build_number := ""%string.
+  Definition build_tag := ""%string.
+  Definition arch := "x86"%string.
+  Definition model := "32sse2"%string.
+  Definition abi := "standard"%string.
+  Definition bitsize := 32.
+  Definition big_endian := false.
+  Definition source_file := "/home/nika/asn1c/skeletons/BOOLEAN.c"%string.
+  Definition normalized := true.
+End Info.
+
+Definition _ASN__PRIMITIVE_TYPE_free : ident := 154%positive.
+Definition _BOOLEAN__xer_body_decode : ident := 192%positive.
+Definition _BOOLEAN_compare : ident := 169%positive.
+Definition _BOOLEAN_decode_ber : ident := 168%positive.
+Definition _BOOLEAN_decode_oer : ident := 164%positive.
+Definition _BOOLEAN_decode_uper : ident := 162%positive.
+Definition _BOOLEAN_decode_xer : ident := 166%positive.
+Definition _BOOLEAN_encode_der : ident := 167%positive.
+Definition _BOOLEAN_encode_oer : ident := 163%positive.
+Definition _BOOLEAN_encode_uper : ident := 161%positive.
+Definition _BOOLEAN_encode_xer : ident := 165%positive.
+Definition _BOOLEAN_free : ident := 171%positive.
+Definition _BOOLEAN_print : ident := 170%positive.
+Definition _BOOLEAN_random_fill : ident := 160%positive.
+Definition ___builtin_ais_annot : ident := 87%positive.
+Definition ___builtin_annot : ident := 94%positive.
+Definition ___builtin_annot_intval : ident := 95%positive.
+Definition ___builtin_bswap : ident := 88%positive.
+Definition ___builtin_bswap16 : ident := 90%positive.
+Definition ___builtin_bswap32 : ident := 89%positive.
+Definition ___builtin_bswap64 : ident := 120%positive.
+Definition ___builtin_clz : ident := 121%positive.
+Definition ___builtin_clzl : ident := 122%positive.
+Definition ___builtin_clzll : ident := 123%positive.
+Definition ___builtin_ctz : ident := 124%positive.
+Definition ___builtin_ctzl : ident := 125%positive.
+Definition ___builtin_ctzll : ident := 126%positive.
+Definition ___builtin_debug : ident := 138%positive.
+Definition ___builtin_fabs : ident := 91%positive.
+Definition ___builtin_fmadd : ident := 129%positive.
+Definition ___builtin_fmax : ident := 127%positive.
+Definition ___builtin_fmin : ident := 128%positive.
+Definition ___builtin_fmsub : ident := 130%positive.
+Definition ___builtin_fnmadd : ident := 131%positive.
+Definition ___builtin_fnmsub : ident := 132%positive.
+Definition ___builtin_fsqrt : ident := 92%positive.
+Definition ___builtin_membar : ident := 96%positive.
+Definition ___builtin_memcpy_aligned : ident := 93%positive.
+Definition ___builtin_nop : ident := 137%positive.
+Definition ___builtin_read16_reversed : ident := 133%positive.
+Definition ___builtin_read32_reversed : ident := 134%positive.
+Definition ___builtin_va_arg : ident := 98%positive.
+Definition ___builtin_va_copy : ident := 99%positive.
+Definition ___builtin_va_end : ident := 100%positive.
+Definition ___builtin_va_start : ident := 97%positive.
+Definition ___builtin_write16_reversed : ident := 135%positive.
+Definition ___builtin_write32_reversed : ident := 136%positive.
+Definition ___compcert_i64_dtos : ident := 105%positive.
+Definition ___compcert_i64_dtou : ident := 106%positive.
+Definition ___compcert_i64_sar : ident := 117%positive.
+Definition ___compcert_i64_sdiv : ident := 111%positive.
+Definition ___compcert_i64_shl : ident := 115%positive.
+Definition ___compcert_i64_shr : ident := 116%positive.
+Definition ___compcert_i64_smod : ident := 113%positive.
+Definition ___compcert_i64_smulh : ident := 118%positive.
+Definition ___compcert_i64_stod : ident := 107%positive.
+Definition ___compcert_i64_stof : ident := 109%positive.
+Definition ___compcert_i64_udiv : ident := 112%positive.
+Definition ___compcert_i64_umod : ident := 114%positive.
+Definition ___compcert_i64_umulh : ident := 119%positive.
+Definition ___compcert_i64_utod : ident := 108%positive.
+Definition ___compcert_i64_utof : ident := 110%positive.
+Definition ___compcert_va_composite : ident := 104%positive.
+Definition ___compcert_va_float64 : ident := 103%positive.
+Definition ___compcert_va_int32 : ident := 101%positive.
+Definition ___compcert_va_int64 : ident := 102%positive.
+Definition ___stringlit_1 : ident := 173%positive.
+Definition ___stringlit_2 : ident := 190%positive.
+Definition ___stringlit_3 : ident := 191%positive.
+Definition ___stringlit_4 : ident := 198%positive.
+Definition ___stringlit_5 : ident := 200%positive.
+Definition ___stringlit_6 : ident := 203%positive.
+Definition ___stringlit_7 : ident := 204%positive.
+Definition ___stringlit_8 : ident := 205%positive.
+Definition __res : ident := 174%positive.
+Definition __res__1 : ident := 182%positive.
+Definition _a : ident := 214%positive.
+Definition _all_tags : ident := 72%positive.
+Definition _all_tags_count : ident := 73%positive.
+Definition _app_key : ident := 185%positive.
+Definition _aptr : ident := 212%positive.
+Definition _asn_DEF_BOOLEAN : ident := 172%positive.
+Definition _asn_DEF_BOOLEAN_tags : ident := 158%positive.
+Definition _asn_OP_BOOLEAN : ident := 159%positive.
+Definition _asn_TYPE_descriptor_s : ident := 4%positive.
+Definition _asn_TYPE_member_s : ident := 75%positive.
+Definition _asn_TYPE_operation_s : ident := 63%positive.
+Definition _asn_TYPE_outmost_tag : ident := 153%positive.
+Definition _asn_bit_data_s : ident := 21%positive.
+Definition _asn_bit_outp_s : ident := 28%positive.
+Definition _asn_codec_ctx_s : ident := 2%positive.
+Definition _asn_dec_rval_s : ident := 10%positive.
+Definition _asn_enc_rval_s : ident := 7%positive.
+Definition _asn_encoding_constraints_s : ident := 60%positive.
+Definition _asn_generic_no_constraint : ident := 148%positive.
+Definition _asn_generic_unknown_constraint : ident := 149%positive.
+Definition _asn_get_few_bits : ident := 146%positive.
+Definition _asn_oer_constraint_number_s : ident := 44%positive.
+Definition _asn_oer_constraints_s : ident := 45%positive.
+Definition _asn_per_constraint_s : ident := 34%positive.
+Definition _asn_per_constraints_s : ident := 39%positive.
+Definition _asn_put_few_bits : ident := 147%positive.
+Definition _asn_random_between : ident := 150%positive.
+Definition _asn_random_fill_result_s : ident := 41%positive.
+Definition _asn_struct_ctx_s : ident := 16%positive.
+Definition _asn_type_selector_result_s : ident := 48%positive.
+Definition _b : ident := 215%positive.
+Definition _ber_check_tags : ident := 143%positive.
+Definition _ber_decode_primitive : ident := 155%positive.
+Definition _ber_decoder : ident := 52%positive.
+Definition _bool_value : ident := 177%positive.
+Definition _bptr : ident := 213%positive.
+Definition _buf : ident := 201%positive.
+Definition _buf_ptr : ident := 178%positive.
+Definition _buffer : ident := 17%positive.
+Definition _buflen : ident := 202%positive.
+Definition _calloc : ident := 140%positive.
+Definition _cb : ident := 184%positive.
+Definition _cb_failed : ident := 199%positive.
+Definition _chunk_buf : ident := 187%positive.
+Definition _chunk_size : ident := 188%positive.
+Definition _code : ident := 8%positive.
+Definition _code2value : ident := 38%positive.
+Definition _compare_struct : ident := 51%positive.
+Definition _constraints : ident := 207%positive.
+Definition _consumed : ident := 9%positive.
+Definition _context : ident := 13%positive.
+Definition _default_value_cmp : ident := 85%positive.
+Definition _default_value_set : ident := 86%positive.
+Definition _der_encode_primitive : ident := 156%positive.
+Definition _der_encoder : ident := 53%positive.
+Definition _der_write_tags : ident := 144%positive.
+Definition _effective_bits : ident := 31%positive.
+Definition _elements : ident := 76%positive.
+Definition _elements_count : ident := 77%positive.
+Definition _encoded : ident := 3%positive.
+Definition _encoding_constraints : ident := 74%positive.
+Definition _er : ident := 195%positive.
+Definition _erval : ident := 186%positive.
+Definition _failed_type : ident := 5%positive.
+Definition _flags : ident := 29%positive.
+Definition _flushed_bytes : ident := 27%positive.
+Definition _free : ident := 141%positive.
+Definition _free_struct : ident := 49%positive.
+Definition _general_constraints : ident := 66%positive.
+Definition _ilevel : ident := 194%positive.
+Definition _left : ident := 15%positive.
+Definition _length : ident := 40%positive.
+Definition _lidx : ident := 181%positive.
+Definition _lower_bound : ident := 32%positive.
+Definition _main : ident := 221%positive.
+Definition _malloc : ident := 139%positive.
+Definition _max_length : ident := 216%positive.
+Definition _max_stack_size : ident := 1%positive.
+Definition _memb_offset : ident := 80%positive.
+Definition _memset : ident := 142%positive.
+Definition _method : ident := 206%positive.
+Definition _moved : ident := 20%positive.
+Definition _name : ident := 67%positive.
+Definition _nbits : ident := 19%positive.
+Definition _nboff : ident := 18%positive.
+Definition _oer_constraints : ident := 64%positive.
+Definition _oer_decode_primitive : ident := 151%positive.
+Definition _oer_decoder : ident := 56%positive.
+Definition _oer_encode_primitive : ident := 152%positive.
+Definition _oer_encoder : ident := 57%positive.
+Definition _ok : ident := 211%positive.
+Definition _op : ident := 69%positive.
+Definition _op_key : ident := 26%positive.
+Definition _opt_codec_ctx : ident := 175%positive.
+Definition _opt_mname : ident := 193%positive.
+Definition _optional : ident := 79%positive.
+Definition _outmost_tag : ident := 62%positive.
+Definition _output : ident := 25%positive.
+Definition _p : ident := 189%positive.
+Definition _pc : ident := 220%positive.
+Definition _pd : ident := 208%positive.
+Definition _per_constraints : ident := 65%positive.
+Definition _phase : ident := 11%positive.
+Definition _po : ident := 210%positive.
+Definition _positive : ident := 43%positive.
+Definition _presence_index : ident := 47%positive.
+Definition _print_struct : ident := 50%positive.
+Definition _ptr : ident := 14%positive.
+Definition _random_fill : ident := 61%positive.
+Definition _range_bits : ident := 30%positive.
+Definition _refill : ident := 22%positive.
+Definition _refill_key : ident := 23%positive.
+Definition _result_failed : ident := 218%positive.
+Definition _result_ok : ident := 217%positive.
+Definition _result_skipped : ident := 219%positive.
+Definition _rv : ident := 209%positive.
+Definition _rval : ident := 180%positive.
+Definition _size : ident := 36%positive.
+Definition _specifics : ident := 78%positive.
+Definition _sptr : ident := 183%positive.
+Definition _st : ident := 179%positive.
+Definition _step : ident := 12%positive.
+Definition _structure_ptr : ident := 6%positive.
+Definition _tag : ident := 81%positive.
+Definition _tag_mode : ident := 82%positive.
+Definition _tags : ident := 70%positive.
+Definition _tags_count : ident := 71%positive.
+Definition _td : ident := 176%positive.
+Definition _tmp_error : ident := 196%positive.
+Definition _tmp_error__1 : ident := 197%positive.
+Definition _tmpspace : ident := 24%positive.
+Definition _type : ident := 83%positive.
+Definition _type_descriptor : ident := 46%positive.
+Definition _type_selector : ident := 84%positive.
+Definition _uper_decoder : ident := 58%positive.
+Definition _uper_encoder : ident := 59%positive.
+Definition _upper_bound : ident := 33%positive.
+Definition _value : ident := 35%positive.
+Definition _value2code : ident := 37%positive.
+Definition _width : ident := 42%positive.
+Definition _xer_check_tag : ident := 145%positive.
+Definition _xer_decode_primitive : ident := 157%positive.
+Definition _xer_decoder : ident := 54%positive.
+Definition _xer_encoder : ident := 55%positive.
+Definition _xml_tag : ident := 68%positive.
+Definition _t'1 : ident := 222%positive.
+Definition _t'10 : ident := 231%positive.
+Definition _t'11 : ident := 232%positive.
+Definition _t'12 : ident := 233%positive.
+Definition _t'13 : ident := 234%positive.
+Definition _t'14 : ident := 235%positive.
+Definition _t'2 : ident := 223%positive.
+Definition _t'3 : ident := 224%positive.
+Definition _t'4 : ident := 225%positive.
+Definition _t'5 : ident := 226%positive.
+Definition _t'6 : ident := 227%positive.
+Definition _t'7 : ident := 228%positive.
+Definition _t'8 : ident := 229%positive.
+Definition _t'9 : ident := 230%positive.
+
+Definition v___stringlit_1 := {|
+  gvar_info := (tarray tschar 8);
+  gvar_init := (Init_int8 (Int.repr 66) :: Init_int8 (Int.repr 79) ::
+                Init_int8 (Int.repr 79) :: Init_int8 (Int.repr 76) ::
+                Init_int8 (Int.repr 69) :: Init_int8 (Int.repr 65) ::
+                Init_int8 (Int.repr 78) :: Init_int8 (Int.repr 0) :: nil);
+  gvar_readonly := true;
+  gvar_volatile := false
+|}.
+
+Definition v___stringlit_3 := {|
+  gvar_info := (tarray tschar 5);
+  gvar_init := (Init_int8 (Int.repr 116) :: Init_int8 (Int.repr 114) ::
+                Init_int8 (Int.repr 117) :: Init_int8 (Int.repr 101) ::
+                Init_int8 (Int.repr 0) :: nil);
+  gvar_readonly := true;
+  gvar_volatile := false
+|}.
+
+Definition v___stringlit_4 := {|
+  gvar_info := (tarray tschar 9);
+  gvar_init := (Init_int8 (Int.repr 60) :: Init_int8 (Int.repr 102) ::
+                Init_int8 (Int.repr 97) :: Init_int8 (Int.repr 108) ::
+                Init_int8 (Int.repr 115) :: Init_int8 (Int.repr 101) ::
+                Init_int8 (Int.repr 47) :: Init_int8 (Int.repr 62) ::
+                Init_int8 (Int.repr 0) :: nil);
+  gvar_readonly := true;
+  gvar_volatile := false
+|}.
+
+Definition v___stringlit_7 := {|
+  gvar_info := (tarray tschar 6);
+  gvar_init := (Init_int8 (Int.repr 70) :: Init_int8 (Int.repr 65) ::
+                Init_int8 (Int.repr 76) :: Init_int8 (Int.repr 83) ::
+                Init_int8 (Int.repr 69) :: Init_int8 (Int.repr 0) :: nil);
+  gvar_readonly := true;
+  gvar_volatile := false
+|}.
+
+Definition v___stringlit_8 := {|
+  gvar_info := (tarray tschar 5);
+  gvar_init := (Init_int8 (Int.repr 84) :: Init_int8 (Int.repr 82) ::
+                Init_int8 (Int.repr 85) :: Init_int8 (Int.repr 69) ::
+                Init_int8 (Int.repr 0) :: nil);
+  gvar_readonly := true;
+  gvar_volatile := false
+|}.
+
+Definition v___stringlit_5 := {|
+  gvar_info := (tarray tschar 8);
+  gvar_init := (Init_int8 (Int.repr 60) :: Init_int8 (Int.repr 116) ::
+                Init_int8 (Int.repr 114) :: Init_int8 (Int.repr 117) ::
+                Init_int8 (Int.repr 101) :: Init_int8 (Int.repr 47) ::
+                Init_int8 (Int.repr 62) :: Init_int8 (Int.repr 0) :: nil);
+  gvar_readonly := true;
+  gvar_volatile := false
+|}.
+
+Definition v___stringlit_2 := {|
+  gvar_info := (tarray tschar 6);
+  gvar_init := (Init_int8 (Int.repr 102) :: Init_int8 (Int.repr 97) ::
+                Init_int8 (Int.repr 108) :: Init_int8 (Int.repr 115) ::
+                Init_int8 (Int.repr 101) :: Init_int8 (Int.repr 0) :: nil);
+  gvar_readonly := true;
+  gvar_volatile := false
+|}.
+
+Definition v___stringlit_6 := {|
+  gvar_info := (tarray tschar 9);
+  gvar_init := (Init_int8 (Int.repr 60) :: Init_int8 (Int.repr 97) ::
+                Init_int8 (Int.repr 98) :: Init_int8 (Int.repr 115) ::
+                Init_int8 (Int.repr 101) :: Init_int8 (Int.repr 110) ::
+                Init_int8 (Int.repr 116) :: Init_int8 (Int.repr 62) ::
+                Init_int8 (Int.repr 0) :: nil);
+  gvar_readonly := true;
+  gvar_volatile := false
+|}.
+
+Definition v_asn_DEF_BOOLEAN_tags := {|
+  gvar_info := (tarray tuint 1);
+  gvar_init := (Init_int32 (Int.repr 4) :: nil);
+  gvar_readonly := true;
+  gvar_volatile := false
+|}.
+
+Definition v_asn_OP_BOOLEAN := {|
+  gvar_info := (Tstruct _asn_TYPE_operation_s noattr);
+  gvar_init := (Init_addrof _BOOLEAN_free (Ptrofs.repr 0) ::
+                Init_addrof _BOOLEAN_print (Ptrofs.repr 0) ::
+                Init_addrof _BOOLEAN_compare (Ptrofs.repr 0) ::
+                Init_addrof _BOOLEAN_decode_ber (Ptrofs.repr 0) ::
+                Init_addrof _BOOLEAN_encode_der (Ptrofs.repr 0) ::
+                Init_addrof _BOOLEAN_decode_xer (Ptrofs.repr 0) ::
+                Init_addrof _BOOLEAN_encode_xer (Ptrofs.repr 0) ::
+                Init_addrof _BOOLEAN_decode_oer (Ptrofs.repr 0) ::
+                Init_addrof _BOOLEAN_encode_oer (Ptrofs.repr 0) ::
+                Init_addrof _BOOLEAN_decode_uper (Ptrofs.repr 0) ::
+                Init_addrof _BOOLEAN_encode_uper (Ptrofs.repr 0) ::
+                Init_addrof _BOOLEAN_random_fill (Ptrofs.repr 0) ::
+                Init_int32 (Int.repr 0) :: nil);
+  gvar_readonly := false;
+  gvar_volatile := false
+|}.
+
+Definition v_asn_DEF_BOOLEAN := {|
+  gvar_info := (Tstruct _asn_TYPE_descriptor_s noattr);
+  gvar_init := (Init_addrof ___stringlit_1 (Ptrofs.repr 0) ::
+                Init_addrof ___stringlit_1 (Ptrofs.repr 0) ::
+                Init_addrof _asn_OP_BOOLEAN (Ptrofs.repr 0) ::
+                Init_addrof _asn_DEF_BOOLEAN_tags (Ptrofs.repr 0) ::
+                Init_int32 (Int.repr 1) ::
+                Init_addrof _asn_DEF_BOOLEAN_tags (Ptrofs.repr 0) ::
+                Init_int32 (Int.repr 1) :: Init_int32 (Int.repr 0) ::
+                Init_int32 (Int.repr 0) ::
+                Init_addrof _asn_generic_no_constraint (Ptrofs.repr 0) ::
+                Init_int32 (Int.repr 0) :: Init_int32 (Int.repr 0) ::
+                Init_int32 (Int.repr 0) :: nil);
+  gvar_readonly := false;
+  gvar_volatile := false
+|}.
+
+Definition f_BOOLEAN_decode_ber := {|
+  fn_return := tvoid;
+  fn_callconv := {|cc_vararg:=false; cc_unproto:=false; cc_structret:=true|};
+  fn_params := ((__res, (tptr (Tstruct _asn_dec_rval_s noattr))) ::
+                (_opt_codec_ctx, (tptr (Tstruct _asn_codec_ctx_s noattr))) ::
+                (_td, (tptr (Tstruct _asn_TYPE_descriptor_s noattr))) ::
+                (_bool_value, (tptr (tptr tvoid))) ::
+                (_buf_ptr, (tptr tvoid)) :: (_size, tuint) ::
+                (_tag_mode, tint) :: nil);
+  fn_vars := ((_rval, (Tstruct _asn_dec_rval_s noattr)) :: (_length, tint) ::
+              (__res__1, (Tstruct _asn_dec_rval_s noattr)) :: nil);
+  fn_temps := ((_st, (tptr tint)) :: (_lidx, tint) :: (_t'3, tint) ::
+               (_t'2, (tptr tvoid)) :: (_t'1, (tptr tvoid)) ::
+               (_t'14, (tptr tvoid)) :: (_t'13, tint) :: (_t'12, tuint) ::
+               (_t'11, tuint) :: (_t'10, tint) :: (_t'9, tint) ::
+               (_t'8, tint) :: (_t'7, tuchar) :: (_t'6, tint) ::
+               (_t'5, tint) :: (_t'4, tuint) :: nil);
+  fn_body :=
+(Ssequence
+  (Ssequence
+    (Sset _t'14
+      (Ederef (Etempvar _bool_value (tptr (tptr tvoid))) (tptr tvoid)))
+    (Sset _st (Ecast (Etempvar _t'14 (tptr tvoid)) (tptr tint))))
+  (Ssequence
+    (Sifthenelse (Ebinop Oeq (Etempvar _st (tptr tint))
+                   (Ecast (Econst_int (Int.repr 0) tint) (tptr tvoid)) tint)
+      (Ssequence
+        (Ssequence
+          (Ssequence
+            (Ssequence
+              (Scall (Some _t'1)
+                (Evar _calloc (Tfunction (Tcons tuint (Tcons tuint Tnil))
+                                (tptr tvoid) cc_default))
+                ((Econst_int (Int.repr 1) tint) :: (Esizeof tint tuint) ::
+                 nil))
+              (Sset _t'2 (Ecast (Etempvar _t'1 (tptr tvoid)) (tptr tvoid))))
+            (Sassign
+              (Ederef (Etempvar _bool_value (tptr (tptr tvoid)))
+                (tptr tvoid)) (Etempvar _t'2 (tptr tvoid))))
+          (Sset _st (Ecast (Etempvar _t'2 (tptr tvoid)) (tptr tint))))
+        (Sifthenelse (Ebinop Oeq (Etempvar _st (tptr tint))
+                       (Ecast (Econst_int (Int.repr 0) tint) (tptr tvoid))
+                       tint)
+          (Ssequence
+            (Sassign
+              (Efield (Evar _rval (Tstruct _asn_dec_rval_s noattr)) _code
+                tint) (Econst_int (Int.repr 2) tint))
+            (Ssequence
+              (Sassign
+                (Efield (Evar _rval (Tstruct _asn_dec_rval_s noattr))
+                  _consumed tuint) (Econst_int (Int.repr 0) tint))
+              (Ssequence
+                (Sassign
+                  (Ederef
+                    (Etempvar __res (tptr (Tstruct _asn_dec_rval_s noattr)))
+                    (Tstruct _asn_dec_rval_s noattr))
+                  (Evar _rval (Tstruct _asn_dec_rval_s noattr)))
+                (Sreturn None))))
+          Sskip))
+      Sskip)
+    (Ssequence
+      (Sloop Sskip Sbreak)
+      (Ssequence
+        (Ssequence
+          (Scall None
+            (Evar _ber_check_tags (Tfunction
+                                    (Tcons
+                                      (tptr (Tstruct _asn_dec_rval_s noattr))
+                                      (Tcons
+                                        (tptr (Tstruct _asn_codec_ctx_s noattr))
+                                        (Tcons
+                                          (tptr (Tstruct _asn_TYPE_descriptor_s noattr))
+                                          (Tcons
+                                            (tptr (Tstruct _asn_struct_ctx_s noattr))
+                                            (Tcons (tptr tvoid)
+                                              (Tcons tuint
+                                                (Tcons tint
+                                                  (Tcons tint
+                                                    (Tcons (tptr tint)
+                                                      (Tcons (tptr tint)
+                                                        Tnil)))))))))) tvoid
+                                    {|cc_vararg:=false; cc_unproto:=false; cc_structret:=true|}))
+            ((Eaddrof (Evar __res__1 (Tstruct _asn_dec_rval_s noattr))
+               (tptr (Tstruct _asn_dec_rval_s noattr))) ::
+             (Etempvar _opt_codec_ctx (tptr (Tstruct _asn_codec_ctx_s noattr))) ::
+             (Etempvar _td (tptr (Tstruct _asn_TYPE_descriptor_s noattr))) ::
+             (Econst_int (Int.repr 0) tint) ::
+             (Etempvar _buf_ptr (tptr tvoid)) :: (Etempvar _size tuint) ::
+             (Etempvar _tag_mode tint) :: (Econst_int (Int.repr 0) tint) ::
+             (Eaddrof (Evar _length tint) (tptr tint)) ::
+             (Econst_int (Int.repr 0) tint) :: nil))
+          (Sassign (Evar _rval (Tstruct _asn_dec_rval_s noattr))
+            (Evar __res__1 (Tstruct _asn_dec_rval_s noattr))))
+        (Ssequence
+          (Ssequence
+            (Sset _t'13
+              (Efield (Evar _rval (Tstruct _asn_dec_rval_s noattr)) _code
+                tint))
+            (Sifthenelse (Ebinop One (Etempvar _t'13 tint)
+                           (Econst_int (Int.repr 0) tint) tint)
+              (Ssequence
+                (Sassign
+                  (Ederef
+                    (Etempvar __res (tptr (Tstruct _asn_dec_rval_s noattr)))
+                    (Tstruct _asn_dec_rval_s noattr))
+                  (Evar _rval (Tstruct _asn_dec_rval_s noattr)))
+                (Sreturn None))
+              Sskip))
+          (Ssequence
+            (Sloop Sskip Sbreak)
+            (Ssequence
+              (Ssequence
+                (Sset _t'12
+                  (Efield (Evar _rval (Tstruct _asn_dec_rval_s noattr))
+                    _consumed tuint))
+                (Sset _buf_ptr
+                  (Ebinop Oadd
+                    (Ecast (Etempvar _buf_ptr (tptr tvoid)) (tptr tschar))
+                    (Etempvar _t'12 tuint) (tptr tschar))))
+              (Ssequence
+                (Ssequence
+                  (Sset _t'11
+                    (Efield (Evar _rval (Tstruct _asn_dec_rval_s noattr))
+                      _consumed tuint))
+                  (Sset _size
+                    (Ebinop Osub (Etempvar _size tuint)
+                      (Etempvar _t'11 tuint) tuint)))
+                (Ssequence
+                  (Ssequence
+                    (Sset _t'10 (Evar _length tint))
+                    (Sifthenelse (Ebinop Ogt (Etempvar _t'10 tint)
+                                   (Ecast (Etempvar _size tuint) tint) tint)
+                      (Ssequence
+                        (Sassign
+                          (Efield
+                            (Evar _rval (Tstruct _asn_dec_rval_s noattr))
+                            _code tint) (Econst_int (Int.repr 1) tint))
+                        (Ssequence
+                          (Sassign
+                            (Efield
+                              (Evar _rval (Tstruct _asn_dec_rval_s noattr))
+                              _consumed tuint)
+                            (Econst_int (Int.repr 0) tint))
+                          (Ssequence
+                            (Sassign
+                              (Ederef
+                                (Etempvar __res (tptr (Tstruct _asn_dec_rval_s noattr)))
+                                (Tstruct _asn_dec_rval_s noattr))
+                              (Evar _rval (Tstruct _asn_dec_rval_s noattr)))
+                            (Sreturn None))))
+                      Sskip))
+                  (Ssequence
+                    (Ssequence
+                      (Ssequence
+                        (Sassign (Ederef (Etempvar _st (tptr tint)) tint)
+                          (Econst_int (Int.repr 0) tint))
+                        (Sset _lidx (Econst_int (Int.repr 0) tint)))
+                      (Sloop
+                        (Ssequence
+                          (Ssequence
+                            (Ssequence
+                              (Sset _t'8 (Evar _length tint))
+                              (Sifthenelse (Ebinop Olt (Etempvar _lidx tint)
+                                             (Etempvar _t'8 tint) tint)
+                                (Ssequence
+                                  (Sset _t'9
+                                    (Ederef (Etempvar _st (tptr tint)) tint))
+                                  (Sset _t'3
+                                    (Ecast
+                                      (Ebinop Oeq (Etempvar _t'9 tint)
+                                        (Econst_int (Int.repr 0) tint) tint)
+                                      tbool)))
+                                (Sset _t'3 (Econst_int (Int.repr 0) tint))))
+                            (Sifthenelse (Etempvar _t'3 tint) Sskip Sbreak))
+                          (Ssequence
+                            (Sset _t'6
+                              (Ederef (Etempvar _st (tptr tint)) tint))
+                            (Ssequence
+                              (Sset _t'7
+                                (Ederef
+                                  (Ebinop Oadd
+                                    (Ecast (Etempvar _buf_ptr (tptr tvoid))
+                                      (tptr tuchar)) (Etempvar _lidx tint)
+                                    (tptr tuchar)) tuchar))
+                              (Sassign
+                                (Ederef (Etempvar _st (tptr tint)) tint)
+                                (Ebinop Oor (Etempvar _t'6 tint)
+                                  (Etempvar _t'7 tuchar) tint)))))
+                        (Sset _lidx
+                          (Ebinop Oadd (Etempvar _lidx tint)
+                            (Econst_int (Int.repr 1) tint) tint))))
+                    (Ssequence
+                      (Sassign
+                        (Efield (Evar _rval (Tstruct _asn_dec_rval_s noattr))
+                          _code tint) (Econst_int (Int.repr 0) tint))
+                      (Ssequence
+                        (Ssequence
+                          (Sset _t'4
+                            (Efield
+                              (Evar _rval (Tstruct _asn_dec_rval_s noattr))
+                              _consumed tuint))
+                          (Ssequence
+                            (Sset _t'5 (Evar _length tint))
+                            (Sassign
+                              (Efield
+                                (Evar _rval (Tstruct _asn_dec_rval_s noattr))
+                                _consumed tuint)
+                              (Ebinop Oadd (Etempvar _t'4 tuint)
+                                (Etempvar _t'5 tint) tuint))))
+                        (Ssequence
+                          (Sloop Sskip Sbreak)
+                          (Ssequence
+                            (Sassign
+                              (Ederef
+                                (Etempvar __res (tptr (Tstruct _asn_dec_rval_s noattr)))
+                                (Tstruct _asn_dec_rval_s noattr))
+                              (Evar _rval (Tstruct _asn_dec_rval_s noattr)))
+                            (Sreturn None)))))))))))))))
+|}.
+
+Definition f_BOOLEAN_encode_der := {|
+  fn_return := tvoid;
+  fn_callconv := {|cc_vararg:=false; cc_unproto:=false; cc_structret:=true|};
+  fn_params := ((__res, (tptr (Tstruct _asn_enc_rval_s noattr))) ::
+                (_td, (tptr (Tstruct _asn_TYPE_descriptor_s noattr))) ::
+                (_sptr, (tptr tvoid)) :: (_tag_mode, tint) ::
+                (_tag, tuint) ::
+                (_cb,
+                 (tptr (Tfunction
+                         (Tcons (tptr tvoid)
+                           (Tcons tuint (Tcons (tptr tvoid) Tnil))) tint
+                         cc_default))) :: (_app_key, (tptr tvoid)) :: nil);
+  fn_vars := ((_erval, (Tstruct _asn_enc_rval_s noattr)) ::
+              (_bool_value, tuchar) :: nil);
+  fn_temps := ((_st, (tptr tint)) :: (_t'3, tint) :: (_t'2, tint) ::
+               (_t'1, tint) :: (_t'6, tint) :: (_t'5, tint) ::
+               (_t'4, tint) :: nil);
+  fn_body :=
+(Ssequence
+  (Sset _st (Ecast (Etempvar _sptr (tptr tvoid)) (tptr tint)))
+  (Ssequence
+    (Ssequence
+      (Scall (Some _t'1)
+        (Evar _der_write_tags (Tfunction
+                                (Tcons
+                                  (tptr (Tstruct _asn_TYPE_descriptor_s noattr))
+                                  (Tcons tuint
+                                    (Tcons tint
+                                      (Tcons tint
+                                        (Tcons tuint
+                                          (Tcons
+                                            (tptr (Tfunction
+                                                    (Tcons (tptr tvoid)
+                                                      (Tcons tuint
+                                                        (Tcons (tptr tvoid)
+                                                          Tnil))) tint
+                                                    cc_default))
+                                            (Tcons (tptr tvoid) Tnil)))))))
+                                tint cc_default))
+        ((Etempvar _td (tptr (Tstruct _asn_TYPE_descriptor_s noattr))) ::
+         (Econst_int (Int.repr 1) tint) :: (Etempvar _tag_mode tint) ::
+         (Econst_int (Int.repr 0) tint) :: (Etempvar _tag tuint) ::
+         (Etempvar _cb (tptr (Tfunction
+                               (Tcons (tptr tvoid)
+                                 (Tcons tuint (Tcons (tptr tvoid) Tnil)))
+                               tint cc_default))) ::
+         (Etempvar _app_key (tptr tvoid)) :: nil))
+      (Sassign
+        (Efield (Evar _erval (Tstruct _asn_enc_rval_s noattr)) _encoded tint)
+        (Etempvar _t'1 tint)))
+    (Ssequence
+      (Ssequence
+        (Sset _t'6
+          (Efield (Evar _erval (Tstruct _asn_enc_rval_s noattr)) _encoded
+            tint))
+        (Sifthenelse (Ebinop Oeq (Etempvar _t'6 tint)
+                       (Eunop Oneg (Econst_int (Int.repr 1) tint) tint) tint)
+          (Ssequence
+            (Sassign
+              (Efield (Evar _erval (Tstruct _asn_enc_rval_s noattr))
+                _failed_type (tptr (Tstruct _asn_TYPE_descriptor_s noattr)))
+              (Etempvar _td (tptr (Tstruct _asn_TYPE_descriptor_s noattr))))
+            (Ssequence
+              (Sassign
+                (Efield (Evar _erval (Tstruct _asn_enc_rval_s noattr))
+                  _structure_ptr (tptr tvoid)) (Etempvar _sptr (tptr tvoid)))
+              (Ssequence
+                (Sassign
+                  (Ederef
+                    (Etempvar __res (tptr (Tstruct _asn_enc_rval_s noattr)))
+                    (Tstruct _asn_enc_rval_s noattr))
+                  (Evar _erval (Tstruct _asn_enc_rval_s noattr)))
+                (Sreturn None))))
+          Sskip))
+      (Ssequence
+        (Sifthenelse (Etempvar _cb (tptr (Tfunction
+                                           (Tcons (tptr tvoid)
+                                             (Tcons tuint
+                                               (Tcons (tptr tvoid) Tnil)))
+                                           tint cc_default)))
+          (Ssequence
+            (Ssequence
+              (Ssequence
+                (Sset _t'5 (Ederef (Etempvar _st (tptr tint)) tint))
+                (Sifthenelse (Etempvar _t'5 tint)
+                  (Sset _t'2 (Ecast (Econst_int (Int.repr 255) tint) tint))
+                  (Sset _t'2 (Ecast (Econst_int (Int.repr 0) tint) tint))))
+              (Sassign (Evar _bool_value tuchar) (Etempvar _t'2 tint)))
+            (Ssequence
+              (Scall (Some _t'3)
+                (Etempvar _cb (tptr (Tfunction
+                                      (Tcons (tptr tvoid)
+                                        (Tcons tuint
+                                          (Tcons (tptr tvoid) Tnil))) tint
+                                      cc_default)))
+                ((Eaddrof (Evar _bool_value tuchar) (tptr tuchar)) ::
+                 (Econst_int (Int.repr 1) tint) ::
+                 (Etempvar _app_key (tptr tvoid)) :: nil))
+              (Sifthenelse (Ebinop Olt (Etempvar _t'3 tint)
+                             (Econst_int (Int.repr 0) tint) tint)
+                (Ssequence
+                  (Sassign
+                    (Efield (Evar _erval (Tstruct _asn_enc_rval_s noattr))
+                      _encoded tint)
+                    (Eunop Oneg (Econst_int (Int.repr 1) tint) tint))
+                  (Ssequence
+                    (Sassign
+                      (Efield (Evar _erval (Tstruct _asn_enc_rval_s noattr))
+                        _failed_type
+                        (tptr (Tstruct _asn_TYPE_descriptor_s noattr)))
+                      (Etempvar _td (tptr (Tstruct _asn_TYPE_descriptor_s noattr))))
+                    (Ssequence
+                      (Sassign
+                        (Efield
+                          (Evar _erval (Tstruct _asn_enc_rval_s noattr))
+                          _structure_ptr (tptr tvoid))
+                        (Etempvar _sptr (tptr tvoid)))
+                      (Ssequence
+                        (Sassign
+                          (Ederef
+                            (Etempvar __res (tptr (Tstruct _asn_enc_rval_s noattr)))
+                            (Tstruct _asn_enc_rval_s noattr))
+                          (Evar _erval (Tstruct _asn_enc_rval_s noattr)))
+                        (Sreturn None)))))
+                Sskip)))
+          Sskip)
+        (Ssequence
+          (Ssequence
+            (Sset _t'4
+              (Efield (Evar _erval (Tstruct _asn_enc_rval_s noattr)) _encoded
+                tint))
+            (Sassign
+              (Efield (Evar _erval (Tstruct _asn_enc_rval_s noattr)) _encoded
+                tint)
+              (Ebinop Oadd (Etempvar _t'4 tint)
+                (Econst_int (Int.repr 1) tint) tint)))
+          (Sloop
+            (Ssequence
+              (Sassign
+                (Efield (Evar _erval (Tstruct _asn_enc_rval_s noattr))
+                  _structure_ptr (tptr tvoid))
+                (Econst_int (Int.repr 0) tint))
+              (Ssequence
+                (Sassign
+                  (Efield (Evar _erval (Tstruct _asn_enc_rval_s noattr))
+                    _failed_type
+                    (tptr (Tstruct _asn_TYPE_descriptor_s noattr)))
+                  (Econst_int (Int.repr 0) tint))
+                (Ssequence
+                  (Sassign
+                    (Ederef
+                      (Etempvar __res (tptr (Tstruct _asn_enc_rval_s noattr)))
+                      (Tstruct _asn_enc_rval_s noattr))
+                    (Evar _erval (Tstruct _asn_enc_rval_s noattr)))
+                  (Sreturn None))))
+            Sbreak))))))
+|}.
+
+Definition f_BOOLEAN__xer_body_decode := {|
+  fn_return := tint;
+  fn_callconv := cc_default;
+  fn_params := ((_td, (tptr (Tstruct _asn_TYPE_descriptor_s noattr))) ::
+                (_sptr, (tptr tvoid)) :: (_chunk_buf, (tptr tvoid)) ::
+                (_chunk_size, tuint) :: nil);
+  fn_vars := nil;
+  fn_temps := ((_st, (tptr tint)) :: (_p, (tptr tschar)) :: (_t'3, tint) ::
+               (_t'2, tint) :: (_t'1, tint) :: (_t'4, tschar) :: nil);
+  fn_body :=
+(Ssequence
+  (Sset _st (Ecast (Etempvar _sptr (tptr tvoid)) (tptr tint)))
+  (Ssequence
+    (Sset _p (Ecast (Etempvar _chunk_buf (tptr tvoid)) (tptr tschar)))
+    (Ssequence
+      (Sifthenelse (Etempvar _chunk_size tuint)
+        (Ssequence
+          (Sset _t'4
+            (Ederef
+              (Ebinop Oadd (Etempvar _p (tptr tschar))
+                (Econst_int (Int.repr 0) tint) (tptr tschar)) tschar))
+          (Sset _t'3
+            (Ecast
+              (Ebinop Oeq (Etempvar _t'4 tschar)
+                (Econst_int (Int.repr 60) tint) tint) tbool)))
+        (Sset _t'3 (Econst_int (Int.repr 0) tint)))
+      (Sifthenelse (Etempvar _t'3 tint)
+        (Ssequence
+          (Ssequence
+            (Scall (Some _t'1)
+              (Evar _xer_check_tag (Tfunction
+                                     (Tcons (tptr tvoid)
+                                       (Tcons tint
+                                         (Tcons (tptr tschar) Tnil))) tint
+                                     cc_default))
+              ((Etempvar _chunk_buf (tptr tvoid)) ::
+               (Etempvar _chunk_size tuint) ::
+               (Evar ___stringlit_2 (tarray tschar 6)) :: nil))
+            (Sswitch (Etempvar _t'1 tint)
+              (LScons (Some 3)
+                (Ssequence
+                  (Sassign (Ederef (Etempvar _st (tptr tint)) tint)
+                    (Econst_int (Int.repr 0) tint))
+                  Sbreak)
+                (LScons (Some 7)
+                  (Ssequence
+                    (Ssequence
+                      (Scall (Some _t'2)
+                        (Evar _xer_check_tag (Tfunction
+                                               (Tcons (tptr tvoid)
+                                                 (Tcons tint
+                                                   (Tcons (tptr tschar) Tnil)))
+                                               tint cc_default))
+                        ((Etempvar _chunk_buf (tptr tvoid)) ::
+                         (Etempvar _chunk_size tuint) ::
+                         (Evar ___stringlit_3 (tarray tschar 5)) :: nil))
+                      (Sifthenelse (Ebinop One (Etempvar _t'2 tint)
+                                     (Econst_int (Int.repr 3) tint) tint)
+                        (Sreturn (Some (Econst_int (Int.repr 2) tint)))
+                        Sskip))
+                    (Ssequence
+                      (Sassign (Ederef (Etempvar _st (tptr tint)) tint)
+                        (Econst_int (Int.repr 1) tint))
+                      Sbreak))
+                  (LScons None
+                    (Sreturn (Some (Econst_int (Int.repr 2) tint)))
+                    LSnil)))))
+          (Sreturn (Some (Econst_int (Int.repr 4) tint))))
+        (Sreturn (Some (Econst_int (Int.repr 2) tint)))))))
+|}.
+
+Definition f_BOOLEAN_decode_xer := {|
+  fn_return := tvoid;
+  fn_callconv := {|cc_vararg:=false; cc_unproto:=false; cc_structret:=true|};
+  fn_params := ((__res, (tptr (Tstruct _asn_dec_rval_s noattr))) ::
+                (_opt_codec_ctx, (tptr (Tstruct _asn_codec_ctx_s noattr))) ::
+                (_td, (tptr (Tstruct _asn_TYPE_descriptor_s noattr))) ::
+                (_sptr, (tptr (tptr tvoid))) ::
+                (_opt_mname, (tptr tschar)) :: (_buf_ptr, (tptr tvoid)) ::
+                (_size, tuint) :: nil);
+  fn_vars := ((__res__1, (Tstruct _asn_dec_rval_s noattr)) :: nil);
+  fn_temps := nil;
+  fn_body :=
+(Ssequence
+  (Ssequence
+    (Scall None
+      (Evar _xer_decode_primitive (Tfunction
+                                    (Tcons
+                                      (tptr (Tstruct _asn_dec_rval_s noattr))
+                                      (Tcons
+                                        (tptr (Tstruct _asn_codec_ctx_s noattr))
+                                        (Tcons
+                                          (tptr (Tstruct _asn_TYPE_descriptor_s noattr))
+                                          (Tcons (tptr (tptr tvoid))
+                                            (Tcons tuint
+                                              (Tcons (tptr tschar)
+                                                (Tcons (tptr tvoid)
+                                                  (Tcons tuint
+                                                    (Tcons
+                                                      (tptr (Tfunction
+                                                              (Tcons
+                                                                (tptr (Tstruct _asn_TYPE_descriptor_s noattr))
+                                                                (Tcons
+                                                                  (tptr tvoid)
+                                                                  (Tcons
+                                                                    (tptr tvoid)
+                                                                    (Tcons
+                                                                    tuint
+                                                                    Tnil))))
+                                                              tint
+                                                              cc_default))
+                                                      Tnil))))))))) tvoid
+                                    {|cc_vararg:=false; cc_unproto:=false; cc_structret:=true|}))
+      ((Eaddrof (Evar __res__1 (Tstruct _asn_dec_rval_s noattr))
+         (tptr (Tstruct _asn_dec_rval_s noattr))) ::
+       (Etempvar _opt_codec_ctx (tptr (Tstruct _asn_codec_ctx_s noattr))) ::
+       (Etempvar _td (tptr (Tstruct _asn_TYPE_descriptor_s noattr))) ::
+       (Etempvar _sptr (tptr (tptr tvoid))) :: (Esizeof tint tuint) ::
+       (Etempvar _opt_mname (tptr tschar)) ::
+       (Etempvar _buf_ptr (tptr tvoid)) :: (Etempvar _size tuint) ::
+       (Evar _BOOLEAN__xer_body_decode (Tfunction
+                                         (Tcons
+                                           (tptr (Tstruct _asn_TYPE_descriptor_s noattr))
+                                           (Tcons (tptr tvoid)
+                                             (Tcons (tptr tvoid)
+                                               (Tcons tuint Tnil)))) tint
+                                         cc_default)) :: nil))
+    (Sassign
+      (Ederef (Etempvar __res (tptr (Tstruct _asn_dec_rval_s noattr)))
+        (Tstruct _asn_dec_rval_s noattr))
+      (Evar __res__1 (Tstruct _asn_dec_rval_s noattr))))
+  (Sreturn None))
+|}.
+
+Definition f_BOOLEAN_encode_xer := {|
+  fn_return := tvoid;
+  fn_callconv := {|cc_vararg:=false; cc_unproto:=false; cc_structret:=true|};
+  fn_params := ((__res, (tptr (Tstruct _asn_enc_rval_s noattr))) ::
+                (_td, (tptr (Tstruct _asn_TYPE_descriptor_s noattr))) ::
+                (_sptr, (tptr tvoid)) :: (_ilevel, tint) :: (_flags, tint) ::
+                (_cb,
+                 (tptr (Tfunction
+                         (Tcons (tptr tvoid)
+                           (Tcons tuint (Tcons (tptr tvoid) Tnil))) tint
+                         cc_default))) :: (_app_key, (tptr tvoid)) :: nil);
+  fn_vars := ((_er, (Tstruct _asn_enc_rval_s noattr)) ::
+              (_tmp_error, (Tstruct _asn_enc_rval_s noattr)) ::
+              (_tmp_error__1, (Tstruct _asn_enc_rval_s noattr)) :: nil);
+  fn_temps := ((_st, (tptr tint)) :: (_t'2, tint) :: (_t'1, tint) ::
+               (_t'5, tint) :: (_t'4, tint) :: (_t'3, tint) :: nil);
+  fn_body :=
+(Ssequence
+  (Sset _st (Ecast (Etempvar _sptr (tptr tvoid)) (tptr tint)))
+  (Ssequence
+    (Sassign
+      (Efield (Evar _er (Tstruct _asn_enc_rval_s noattr)) _encoded tint)
+      (Econst_int (Int.repr 0) tint))
+    (Ssequence
+      (Sassign
+        (Efield (Evar _er (Tstruct _asn_enc_rval_s noattr)) _failed_type
+          (tptr (Tstruct _asn_TYPE_descriptor_s noattr)))
+        (Econst_int (Int.repr 0) tint))
+      (Ssequence
+        (Sassign
+          (Efield (Evar _er (Tstruct _asn_enc_rval_s noattr)) _structure_ptr
+            (tptr tvoid)) (Econst_int (Int.repr 0) tint))
+        (Ssequence
+          (Sifthenelse (Eunop Onotbool (Etempvar _st (tptr tint)) tint)
+            (Sloop
+              (Ssequence
+                (Sassign
+                  (Efield (Evar _tmp_error (Tstruct _asn_enc_rval_s noattr))
+                    _encoded tint)
+                  (Eunop Oneg (Econst_int (Int.repr 1) tint) tint))
+                (Ssequence
+                  (Sassign
+                    (Efield
+                      (Evar _tmp_error (Tstruct _asn_enc_rval_s noattr))
+                      _failed_type
+                      (tptr (Tstruct _asn_TYPE_descriptor_s noattr)))
+                    (Etempvar _td (tptr (Tstruct _asn_TYPE_descriptor_s noattr))))
+                  (Ssequence
+                    (Sassign
+                      (Efield
+                        (Evar _tmp_error (Tstruct _asn_enc_rval_s noattr))
+                        _structure_ptr (tptr tvoid))
+                      (Etempvar _sptr (tptr tvoid)))
+                    (Ssequence
+                      (Sloop Sskip Sbreak)
+                      (Ssequence
+                        (Sassign
+                          (Ederef
+                            (Etempvar __res (tptr (Tstruct _asn_enc_rval_s noattr)))
+                            (Tstruct _asn_enc_rval_s noattr))
+                          (Evar _tmp_error (Tstruct _asn_enc_rval_s noattr)))
+                        (Sreturn None))))))
+              Sbreak)
+            Sskip)
+          (Ssequence
+            (Ssequence
+              (Sset _t'3 (Ederef (Etempvar _st (tptr tint)) tint))
+              (Sifthenelse (Etempvar _t'3 tint)
+                (Sloop
+                  (Ssequence
+                    (Ssequence
+                      (Scall (Some _t'1)
+                        (Etempvar _cb (tptr (Tfunction
+                                              (Tcons (tptr tvoid)
+                                                (Tcons tuint
+                                                  (Tcons (tptr tvoid) Tnil)))
+                                              tint cc_default)))
+                        ((Evar ___stringlit_5 (tarray tschar 8)) ::
+                         (Econst_int (Int.repr 7) tint) ::
+                         (Etempvar _app_key (tptr tvoid)) :: nil))
+                      (Sifthenelse (Ebinop Olt (Etempvar _t'1 tint)
+                                     (Econst_int (Int.repr 0) tint) tint)
+                        (Sgoto _cb_failed)
+                        Sskip))
+                    (Ssequence
+                      (Sset _t'5
+                        (Efield (Evar _er (Tstruct _asn_enc_rval_s noattr))
+                          _encoded tint))
+                      (Sassign
+                        (Efield (Evar _er (Tstruct _asn_enc_rval_s noattr))
+                          _encoded tint)
+                        (Ebinop Oadd (Etempvar _t'5 tint)
+                          (Econst_int (Int.repr 7) tint) tint))))
+                  Sbreak)
+                (Sloop
+                  (Ssequence
+                    (Ssequence
+                      (Scall (Some _t'2)
+                        (Etempvar _cb (tptr (Tfunction
+                                              (Tcons (tptr tvoid)
+                                                (Tcons tuint
+                                                  (Tcons (tptr tvoid) Tnil)))
+                                              tint cc_default)))
+                        ((Evar ___stringlit_4 (tarray tschar 9)) ::
+                         (Econst_int (Int.repr 8) tint) ::
+                         (Etempvar _app_key (tptr tvoid)) :: nil))
+                      (Sifthenelse (Ebinop Olt (Etempvar _t'2 tint)
+                                     (Econst_int (Int.repr 0) tint) tint)
+                        (Sgoto _cb_failed)
+                        Sskip))
+                    (Ssequence
+                      (Sset _t'4
+                        (Efield (Evar _er (Tstruct _asn_enc_rval_s noattr))
+                          _encoded tint))
+                      (Sassign
+                        (Efield (Evar _er (Tstruct _asn_enc_rval_s noattr))
+                          _encoded tint)
+                        (Ebinop Oadd (Etempvar _t'4 tint)
+                          (Econst_int (Int.repr 8) tint) tint))))
+                  Sbreak)))
+            (Ssequence
+              (Sloop
+                (Ssequence
+                  (Sassign
+                    (Efield (Evar _er (Tstruct _asn_enc_rval_s noattr))
+                      _structure_ptr (tptr tvoid))
+                    (Econst_int (Int.repr 0) tint))
+                  (Ssequence
+                    (Sassign
+                      (Efield (Evar _er (Tstruct _asn_enc_rval_s noattr))
+                        _failed_type
+                        (tptr (Tstruct _asn_TYPE_descriptor_s noattr)))
+                      (Econst_int (Int.repr 0) tint))
+                    (Ssequence
+                      (Sassign
+                        (Ederef
+                          (Etempvar __res (tptr (Tstruct _asn_enc_rval_s noattr)))
+                          (Tstruct _asn_enc_rval_s noattr))
+                        (Evar _er (Tstruct _asn_enc_rval_s noattr)))
+                      (Sreturn None))))
+                Sbreak)
+              (Slabel _cb_failed
+                (Sloop
+                  (Ssequence
+                    (Sassign
+                      (Efield
+                        (Evar _tmp_error__1 (Tstruct _asn_enc_rval_s noattr))
+                        _encoded tint)
+                      (Eunop Oneg (Econst_int (Int.repr 1) tint) tint))
+                    (Ssequence
+                      (Sassign
+                        (Efield
+                          (Evar _tmp_error__1 (Tstruct _asn_enc_rval_s noattr))
+                          _failed_type
+                          (tptr (Tstruct _asn_TYPE_descriptor_s noattr)))
+                        (Etempvar _td (tptr (Tstruct _asn_TYPE_descriptor_s noattr))))
+                      (Ssequence
+                        (Sassign
+                          (Efield
+                            (Evar _tmp_error__1 (Tstruct _asn_enc_rval_s noattr))
+                            _structure_ptr (tptr tvoid))
+                          (Etempvar _sptr (tptr tvoid)))
+                        (Ssequence
+                          (Sloop Sskip Sbreak)
+                          (Ssequence
+                            (Sassign
+                              (Ederef
+                                (Etempvar __res (tptr (Tstruct _asn_enc_rval_s noattr)))
+                                (Tstruct _asn_enc_rval_s noattr))
+                              (Evar _tmp_error__1 (Tstruct _asn_enc_rval_s noattr)))
+                            (Sreturn None))))))
+                  Sbreak)))))))))
+|}.
+
+Definition f_BOOLEAN_print := {|
+  fn_return := tint;
+  fn_callconv := cc_default;
+  fn_params := ((_td, (tptr (Tstruct _asn_TYPE_descriptor_s noattr))) ::
+                (_sptr, (tptr tvoid)) :: (_ilevel, tint) ::
+                (_cb,
+                 (tptr (Tfunction
+                         (Tcons (tptr tvoid)
+                           (Tcons tuint (Tcons (tptr tvoid) Tnil))) tint
+                         cc_default))) :: (_app_key, (tptr tvoid)) :: nil);
+  fn_vars := nil;
+  fn_temps := ((_st, (tptr tint)) :: (_buf, (tptr tschar)) ::
+               (_buflen, tuint) :: (_t'2, tint) :: (_t'1, tint) ::
+               (_t'3, tint) :: nil);
+  fn_body :=
+(Ssequence
+  (Sset _st (Ecast (Etempvar _sptr (tptr tvoid)) (tptr tint)))
+  (Ssequence
+    (Sifthenelse (Etempvar _st (tptr tint))
+      (Ssequence
+        (Sset _t'3 (Ederef (Etempvar _st (tptr tint)) tint))
+        (Sifthenelse (Etempvar _t'3 tint)
+          (Ssequence
+            (Sset _buf (Evar ___stringlit_8 (tarray tschar 5)))
+            (Sset _buflen (Econst_int (Int.repr 4) tint)))
+          (Ssequence
+            (Sset _buf (Evar ___stringlit_7 (tarray tschar 6)))
+            (Sset _buflen (Econst_int (Int.repr 5) tint)))))
+      (Ssequence
+        (Sset _buf (Evar ___stringlit_6 (tarray tschar 9)))
+        (Sset _buflen (Econst_int (Int.repr 8) tint))))
+    (Ssequence
+      (Ssequence
+        (Scall (Some _t'1)
+          (Etempvar _cb (tptr (Tfunction
+                                (Tcons (tptr tvoid)
+                                  (Tcons tuint (Tcons (tptr tvoid) Tnil)))
+                                tint cc_default)))
+          ((Etempvar _buf (tptr tschar)) :: (Etempvar _buflen tuint) ::
+           (Etempvar _app_key (tptr tvoid)) :: nil))
+        (Sifthenelse (Ebinop Olt (Etempvar _t'1 tint)
+                       (Econst_int (Int.repr 0) tint) tint)
+          (Sset _t'2
+            (Ecast (Eunop Oneg (Econst_int (Int.repr 1) tint) tint) tint))
+          (Sset _t'2 (Ecast (Econst_int (Int.repr 0) tint) tint))))
+      (Sreturn (Some (Etempvar _t'2 tint))))))
+|}.
+
+Definition f_BOOLEAN_free := {|
+  fn_return := tvoid;
+  fn_callconv := cc_default;
+  fn_params := ((_td, (tptr (Tstruct _asn_TYPE_descriptor_s noattr))) ::
+                (_ptr, (tptr tvoid)) :: (_method, tint) :: nil);
+  fn_vars := nil;
+  fn_temps := ((_t'1, tint) :: nil);
+  fn_body :=
+(Ssequence
+  (Sifthenelse (Etempvar _td (tptr (Tstruct _asn_TYPE_descriptor_s noattr)))
+    (Sset _t'1 (Ecast (Etempvar _ptr (tptr tvoid)) tbool))
+    (Sset _t'1 (Econst_int (Int.repr 0) tint)))
+  (Sifthenelse (Etempvar _t'1 tint)
+    (Sswitch (Etempvar _method tint)
+      (LScons (Some 0)
+        (Ssequence
+          (Scall None
+            (Evar _free (Tfunction (Tcons (tptr tvoid) Tnil) tvoid
+                          cc_default)) ((Etempvar _ptr (tptr tvoid)) :: nil))
+          Sbreak)
+        (LScons (Some 1)
+          Sbreak
+          (LScons (Some 2)
+            (Ssequence
+              (Scall None
+                (Evar _memset (Tfunction
+                                (Tcons (tptr tvoid)
+                                  (Tcons tint (Tcons tuint Tnil)))
+                                (tptr tvoid) cc_default))
+                ((Etempvar _ptr (tptr tvoid)) ::
+                 (Econst_int (Int.repr 0) tint) :: (Esizeof tint tuint) ::
+                 nil))
+              Sbreak)
+            LSnil))))
+    Sskip))
+|}.
+
+Definition f_BOOLEAN_decode_uper := {|
+  fn_return := tvoid;
+  fn_callconv := {|cc_vararg:=false; cc_unproto:=false; cc_structret:=true|};
+  fn_params := ((__res, (tptr (Tstruct _asn_dec_rval_s noattr))) ::
+                (_opt_codec_ctx, (tptr (Tstruct _asn_codec_ctx_s noattr))) ::
+                (_td, (tptr (Tstruct _asn_TYPE_descriptor_s noattr))) ::
+                (_constraints,
+                 (tptr (Tstruct _asn_per_constraints_s noattr))) ::
+                (_sptr, (tptr (tptr tvoid))) ::
+                (_pd, (tptr (Tstruct _asn_bit_data_s noattr))) :: nil);
+  fn_vars := ((_rv, (Tstruct _asn_dec_rval_s noattr)) ::
+              (_tmp_error, (Tstruct _asn_dec_rval_s noattr)) ::
+              (_tmp_error__1, (Tstruct _asn_dec_rval_s noattr)) :: nil);
+  fn_temps := ((_st, (tptr tint)) :: (_t'3, tint) :: (_t'2, (tptr tvoid)) ::
+               (_t'1, (tptr tvoid)) :: (_t'4, (tptr tvoid)) :: nil);
+  fn_body :=
+(Ssequence
+  (Ssequence
+    (Sset _t'4 (Ederef (Etempvar _sptr (tptr (tptr tvoid))) (tptr tvoid)))
+    (Sset _st (Ecast (Etempvar _t'4 (tptr tvoid)) (tptr tint))))
+  (Ssequence
+    (Sifthenelse (Eunop Onotbool (Etempvar _st (tptr tint)) tint)
+      (Ssequence
+        (Ssequence
+          (Ssequence
+            (Ssequence
+              (Scall (Some _t'1)
+                (Evar _malloc (Tfunction (Tcons tuint Tnil) (tptr tvoid)
+                                cc_default)) ((Esizeof tint tuint) :: nil))
+              (Sset _t'2 (Ecast (Etempvar _t'1 (tptr tvoid)) (tptr tvoid))))
+            (Sassign
+              (Ederef (Etempvar _sptr (tptr (tptr tvoid))) (tptr tvoid))
+              (Etempvar _t'2 (tptr tvoid))))
+          (Sset _st (Ecast (Etempvar _t'2 (tptr tvoid)) (tptr tint))))
+        (Sifthenelse (Eunop Onotbool (Etempvar _st (tptr tint)) tint)
+          (Sloop
+            (Ssequence
+              (Sassign
+                (Efield (Evar _tmp_error (Tstruct _asn_dec_rval_s noattr))
+                  _code tint) (Econst_int (Int.repr 2) tint))
+              (Ssequence
+                (Sassign
+                  (Efield (Evar _tmp_error (Tstruct _asn_dec_rval_s noattr))
+                    _consumed tuint) (Econst_int (Int.repr 0) tint))
+                (Ssequence
+                  (Sloop Sskip Sbreak)
+                  (Ssequence
+                    (Sassign
+                      (Ederef
+                        (Etempvar __res (tptr (Tstruct _asn_dec_rval_s noattr)))
+                        (Tstruct _asn_dec_rval_s noattr))
+                      (Evar _tmp_error (Tstruct _asn_dec_rval_s noattr)))
+                    (Sreturn None)))))
+            Sbreak)
+          Sskip))
+      Sskip)
+    (Ssequence
+      (Ssequence
+        (Scall (Some _t'3)
+          (Evar _asn_get_few_bits (Tfunction
+                                    (Tcons
+                                      (tptr (Tstruct _asn_bit_data_s noattr))
+                                      (Tcons tint Tnil)) tint cc_default))
+          ((Etempvar _pd (tptr (Tstruct _asn_bit_data_s noattr))) ::
+           (Econst_int (Int.repr 1) tint) :: nil))
+        (Sswitch (Etempvar _t'3 tint)
+          (LScons (Some 1)
+            (Ssequence
+              (Sassign (Ederef (Etempvar _st (tptr tint)) tint)
+                (Econst_int (Int.repr 1) tint))
+              Sbreak)
+            (LScons (Some 0)
+              (Ssequence
+                (Sassign (Ederef (Etempvar _st (tptr tint)) tint)
+                  (Econst_int (Int.repr 0) tint))
+                Sbreak)
+              (LScons (Some 4294967295)
+                Sskip
+                (LScons None
+                  (Sloop
+                    (Ssequence
+                      (Sassign
+                        (Efield
+                          (Evar _tmp_error__1 (Tstruct _asn_dec_rval_s noattr))
+                          _code tint) (Econst_int (Int.repr 1) tint))
+                      (Ssequence
+                        (Sassign
+                          (Efield
+                            (Evar _tmp_error__1 (Tstruct _asn_dec_rval_s noattr))
+                            _consumed tuint) (Econst_int (Int.repr 0) tint))
+                        (Ssequence
+                          (Sassign
+                            (Ederef
+                              (Etempvar __res (tptr (Tstruct _asn_dec_rval_s noattr)))
+                              (Tstruct _asn_dec_rval_s noattr))
+                            (Evar _tmp_error__1 (Tstruct _asn_dec_rval_s noattr)))
+                          (Sreturn None))))
+                    Sbreak)
+                  LSnil))))))
+      (Ssequence
+        (Sloop Sskip Sbreak)
+        (Ssequence
+          (Sassign
+            (Efield (Evar _rv (Tstruct _asn_dec_rval_s noattr)) _code tint)
+            (Econst_int (Int.repr 0) tint))
+          (Ssequence
+            (Sassign
+              (Efield (Evar _rv (Tstruct _asn_dec_rval_s noattr)) _consumed
+                tuint) (Econst_int (Int.repr 1) tint))
+            (Ssequence
+              (Sassign
+                (Ederef
+                  (Etempvar __res (tptr (Tstruct _asn_dec_rval_s noattr)))
+                  (Tstruct _asn_dec_rval_s noattr))
+                (Evar _rv (Tstruct _asn_dec_rval_s noattr)))
+              (Sreturn None))))))))
+|}.
+
+Definition f_BOOLEAN_encode_uper := {|
+  fn_return := tvoid;
+  fn_callconv := {|cc_vararg:=false; cc_unproto:=false; cc_structret:=true|};
+  fn_params := ((__res, (tptr (Tstruct _asn_enc_rval_s noattr))) ::
+                (_td, (tptr (Tstruct _asn_TYPE_descriptor_s noattr))) ::
+                (_constraints,
+                 (tptr (Tstruct _asn_per_constraints_s noattr))) ::
+                (_sptr, (tptr tvoid)) ::
+                (_po, (tptr (Tstruct _asn_bit_outp_s noattr))) :: nil);
+  fn_vars := ((_er, (Tstruct _asn_enc_rval_s noattr)) ::
+              (_tmp_error, (Tstruct _asn_enc_rval_s noattr)) ::
+              (_tmp_error__1, (Tstruct _asn_enc_rval_s noattr)) :: nil);
+  fn_temps := ((_st, (tptr tint)) :: (_t'2, tint) :: (_t'1, tint) ::
+               (_t'3, tint) :: nil);
+  fn_body :=
+(Ssequence
+  (Sset _st (Ecast (Etempvar _sptr (tptr tvoid)) (tptr tint)))
+  (Ssequence
+    (Sassign
+      (Efield (Evar _er (Tstruct _asn_enc_rval_s noattr)) _encoded tint)
+      (Econst_int (Int.repr 0) tint))
+    (Ssequence
+      (Sassign
+        (Efield (Evar _er (Tstruct _asn_enc_rval_s noattr)) _failed_type
+          (tptr (Tstruct _asn_TYPE_descriptor_s noattr)))
+        (Econst_int (Int.repr 0) tint))
+      (Ssequence
+        (Sassign
+          (Efield (Evar _er (Tstruct _asn_enc_rval_s noattr)) _structure_ptr
+            (tptr tvoid)) (Econst_int (Int.repr 0) tint))
+        (Ssequence
+          (Sifthenelse (Eunop Onotbool (Etempvar _st (tptr tint)) tint)
+            (Sloop
+              (Ssequence
+                (Sassign
+                  (Efield (Evar _tmp_error (Tstruct _asn_enc_rval_s noattr))
+                    _encoded tint)
+                  (Eunop Oneg (Econst_int (Int.repr 1) tint) tint))
+                (Ssequence
+                  (Sassign
+                    (Efield
+                      (Evar _tmp_error (Tstruct _asn_enc_rval_s noattr))
+                      _failed_type
+                      (tptr (Tstruct _asn_TYPE_descriptor_s noattr)))
+                    (Etempvar _td (tptr (Tstruct _asn_TYPE_descriptor_s noattr))))
+                  (Ssequence
+                    (Sassign
+                      (Efield
+                        (Evar _tmp_error (Tstruct _asn_enc_rval_s noattr))
+                        _structure_ptr (tptr tvoid))
+                      (Etempvar _sptr (tptr tvoid)))
+                    (Ssequence
+                      (Sloop Sskip Sbreak)
+                      (Ssequence
+                        (Sassign
+                          (Ederef
+                            (Etempvar __res (tptr (Tstruct _asn_enc_rval_s noattr)))
+                            (Tstruct _asn_enc_rval_s noattr))
+                          (Evar _tmp_error (Tstruct _asn_enc_rval_s noattr)))
+                        (Sreturn None))))))
+              Sbreak)
+            Sskip)
+          (Ssequence
+            (Ssequence
+              (Ssequence
+                (Ssequence
+                  (Sset _t'3 (Ederef (Etempvar _st (tptr tint)) tint))
+                  (Sifthenelse (Etempvar _t'3 tint)
+                    (Sset _t'1 (Ecast (Econst_int (Int.repr 1) tint) tint))
+                    (Sset _t'1 (Ecast (Econst_int (Int.repr 0) tint) tint))))
+                (Scall (Some _t'2)
+                  (Evar _asn_put_few_bits (Tfunction
+                                            (Tcons
+                                              (tptr (Tstruct _asn_bit_outp_s noattr))
+                                              (Tcons tuint (Tcons tint Tnil)))
+                                            tint cc_default))
+                  ((Etempvar _po (tptr (Tstruct _asn_bit_outp_s noattr))) ::
+                   (Etempvar _t'1 tint) :: (Econst_int (Int.repr 1) tint) ::
+                   nil)))
+              (Sifthenelse (Etempvar _t'2 tint)
+                (Sloop
+                  (Ssequence
+                    (Sassign
+                      (Efield
+                        (Evar _tmp_error__1 (Tstruct _asn_enc_rval_s noattr))
+                        _encoded tint)
+                      (Eunop Oneg (Econst_int (Int.repr 1) tint) tint))
+                    (Ssequence
+                      (Sassign
+                        (Efield
+                          (Evar _tmp_error__1 (Tstruct _asn_enc_rval_s noattr))
+                          _failed_type
+                          (tptr (Tstruct _asn_TYPE_descriptor_s noattr)))
+                        (Etempvar _td (tptr (Tstruct _asn_TYPE_descriptor_s noattr))))
+                      (Ssequence
+                        (Sassign
+                          (Efield
+                            (Evar _tmp_error__1 (Tstruct _asn_enc_rval_s noattr))
+                            _structure_ptr (tptr tvoid))
+                          (Etempvar _sptr (tptr tvoid)))
+                        (Ssequence
+                          (Sloop Sskip Sbreak)
+                          (Ssequence
+                            (Sassign
+                              (Ederef
+                                (Etempvar __res (tptr (Tstruct _asn_enc_rval_s noattr)))
+                                (Tstruct _asn_enc_rval_s noattr))
+                              (Evar _tmp_error__1 (Tstruct _asn_enc_rval_s noattr)))
+                            (Sreturn None))))))
+                  Sbreak)
+                Sskip))
+            (Sloop
+              (Ssequence
+                (Sassign
+                  (Efield (Evar _er (Tstruct _asn_enc_rval_s noattr))
+                    _structure_ptr (tptr tvoid))
+                  (Econst_int (Int.repr 0) tint))
+                (Ssequence
+                  (Sassign
+                    (Efield (Evar _er (Tstruct _asn_enc_rval_s noattr))
+                      _failed_type
+                      (tptr (Tstruct _asn_TYPE_descriptor_s noattr)))
+                    (Econst_int (Int.repr 0) tint))
+                  (Ssequence
+                    (Sassign
+                      (Ederef
+                        (Etempvar __res (tptr (Tstruct _asn_enc_rval_s noattr)))
+                        (Tstruct _asn_enc_rval_s noattr))
+                      (Evar _er (Tstruct _asn_enc_rval_s noattr)))
+                    (Sreturn None))))
+              Sbreak)))))))
+|}.
+
+Definition f_BOOLEAN_encode_oer := {|
+  fn_return := tvoid;
+  fn_callconv := {|cc_vararg:=false; cc_unproto:=false; cc_structret:=true|};
+  fn_params := ((__res, (tptr (Tstruct _asn_enc_rval_s noattr))) ::
+                (_td, (tptr (Tstruct _asn_TYPE_descriptor_s noattr))) ::
+                (_constraints,
+                 (tptr (Tstruct _asn_oer_constraints_s noattr))) ::
+                (_sptr, (tptr tvoid)) ::
+                (_cb,
+                 (tptr (Tfunction
+                         (Tcons (tptr tvoid)
+                           (Tcons tuint (Tcons (tptr tvoid) Tnil))) tint
+                         cc_default))) :: (_app_key, (tptr tvoid)) :: nil);
+  fn_vars := ((_er, (Tstruct _asn_enc_rval_s noattr)) ::
+              (_bool_value, tuchar) ::
+              (_tmp_error, (Tstruct _asn_enc_rval_s noattr)) :: nil);
+  fn_temps := ((_st, (tptr tint)) :: (_t'2, tint) :: (_t'1, tint) ::
+               (_t'3, tint) :: nil);
+  fn_body :=
+(Ssequence
+  (Sassign (Efield (Evar _er (Tstruct _asn_enc_rval_s noattr)) _encoded tint)
+    (Econst_int (Int.repr 1) tint))
+  (Ssequence
+    (Sassign
+      (Efield (Evar _er (Tstruct _asn_enc_rval_s noattr)) _failed_type
+        (tptr (Tstruct _asn_TYPE_descriptor_s noattr)))
+      (Econst_int (Int.repr 0) tint))
+    (Ssequence
+      (Sassign
+        (Efield (Evar _er (Tstruct _asn_enc_rval_s noattr)) _structure_ptr
+          (tptr tvoid)) (Econst_int (Int.repr 0) tint))
+      (Ssequence
+        (Sset _st (Etempvar _sptr (tptr tvoid)))
+        (Ssequence
+          (Ssequence
+            (Ssequence
+              (Sset _t'3 (Ederef (Etempvar _st (tptr tint)) tint))
+              (Sifthenelse (Etempvar _t'3 tint)
+                (Sset _t'1 (Ecast (Econst_int (Int.repr 255) tint) tint))
+                (Sset _t'1 (Ecast (Econst_int (Int.repr 0) tint) tint))))
+            (Sassign (Evar _bool_value tuchar) (Etempvar _t'1 tint)))
+          (Ssequence
+            (Scall (Some _t'2)
+              (Etempvar _cb (tptr (Tfunction
+                                    (Tcons (tptr tvoid)
+                                      (Tcons tuint (Tcons (tptr tvoid) Tnil)))
+                                    tint cc_default)))
+              ((Eaddrof (Evar _bool_value tuchar) (tptr tuchar)) ::
+               (Econst_int (Int.repr 1) tint) ::
+               (Etempvar _app_key (tptr tvoid)) :: nil))
+            (Sifthenelse (Ebinop Olt (Etempvar _t'2 tint)
+                           (Econst_int (Int.repr 0) tint) tint)
+              (Sloop
+                (Ssequence
+                  (Sassign
+                    (Efield
+                      (Evar _tmp_error (Tstruct _asn_enc_rval_s noattr))
+                      _encoded tint)
+                    (Eunop Oneg (Econst_int (Int.repr 1) tint) tint))
+                  (Ssequence
+                    (Sassign
+                      (Efield
+                        (Evar _tmp_error (Tstruct _asn_enc_rval_s noattr))
+                        _failed_type
+                        (tptr (Tstruct _asn_TYPE_descriptor_s noattr)))
+                      (Etempvar _td (tptr (Tstruct _asn_TYPE_descriptor_s noattr))))
+                    (Ssequence
+                      (Sassign
+                        (Efield
+                          (Evar _tmp_error (Tstruct _asn_enc_rval_s noattr))
+                          _structure_ptr (tptr tvoid))
+                        (Etempvar _sptr (tptr tvoid)))
+                      (Ssequence
+                        (Sloop Sskip Sbreak)
+                        (Ssequence
+                          (Sassign
+                            (Ederef
+                              (Etempvar __res (tptr (Tstruct _asn_enc_rval_s noattr)))
+                              (Tstruct _asn_enc_rval_s noattr))
+                            (Evar _tmp_error (Tstruct _asn_enc_rval_s noattr)))
+                          (Sreturn None))))))
+                Sbreak)
+              (Sloop
+                (Ssequence
+                  (Sassign
+                    (Efield (Evar _er (Tstruct _asn_enc_rval_s noattr))
+                      _structure_ptr (tptr tvoid))
+                    (Econst_int (Int.repr 0) tint))
+                  (Ssequence
+                    (Sassign
+                      (Efield (Evar _er (Tstruct _asn_enc_rval_s noattr))
+                        _failed_type
+                        (tptr (Tstruct _asn_TYPE_descriptor_s noattr)))
+                      (Econst_int (Int.repr 0) tint))
+                    (Ssequence
+                      (Sassign
+                        (Ederef
+                          (Etempvar __res (tptr (Tstruct _asn_enc_rval_s noattr)))
+                          (Tstruct _asn_enc_rval_s noattr))
+                        (Evar _er (Tstruct _asn_enc_rval_s noattr)))
+                      (Sreturn None))))
+                Sbreak))))))))
+|}.
+
+Definition f_BOOLEAN_decode_oer := {|
+  fn_return := tvoid;
+  fn_callconv := {|cc_vararg:=false; cc_unproto:=false; cc_structret:=true|};
+  fn_params := ((__res, (tptr (Tstruct _asn_dec_rval_s noattr))) ::
+                (_opt_codec_ctx, (tptr (Tstruct _asn_codec_ctx_s noattr))) ::
+                (_td, (tptr (Tstruct _asn_TYPE_descriptor_s noattr))) ::
+                (_constraints,
+                 (tptr (Tstruct _asn_oer_constraints_s noattr))) ::
+                (_sptr, (tptr (tptr tvoid))) :: (_ptr, (tptr tvoid)) ::
+                (_size, tuint) :: nil);
+  fn_vars := ((_ok, (Tstruct _asn_dec_rval_s noattr)) ::
+              (_tmp_error, (Tstruct _asn_dec_rval_s noattr)) ::
+              (_tmp_error__1, (Tstruct _asn_dec_rval_s noattr)) :: nil);
+  fn_temps := ((_st, (tptr tint)) :: (_t'3, (tptr tint)) ::
+               (_t'2, (tptr tvoid)) :: (_t'1, (tptr tvoid)) ::
+               (_t'5, (tptr tvoid)) :: (_t'4, tuchar) :: nil);
+  fn_body :=
+(Ssequence
+  (Sassign (Efield (Evar _ok (Tstruct _asn_dec_rval_s noattr)) _code tint)
+    (Econst_int (Int.repr 0) tint))
+  (Ssequence
+    (Sassign
+      (Efield (Evar _ok (Tstruct _asn_dec_rval_s noattr)) _consumed tuint)
+      (Econst_int (Int.repr 1) tint))
+    (Ssequence
+      (Sifthenelse (Ebinop Olt (Etempvar _size tuint)
+                     (Econst_int (Int.repr 1) tint) tint)
+        (Sloop
+          (Ssequence
+            (Sassign
+              (Efield (Evar _tmp_error (Tstruct _asn_dec_rval_s noattr))
+                _code tint) (Econst_int (Int.repr 1) tint))
+            (Ssequence
+              (Sassign
+                (Efield (Evar _tmp_error (Tstruct _asn_dec_rval_s noattr))
+                  _consumed tuint) (Econst_int (Int.repr 0) tint))
+              (Ssequence
+                (Sassign
+                  (Ederef
+                    (Etempvar __res (tptr (Tstruct _asn_dec_rval_s noattr)))
+                    (Tstruct _asn_dec_rval_s noattr))
+                  (Evar _tmp_error (Tstruct _asn_dec_rval_s noattr)))
+                (Sreturn None))))
+          Sbreak)
+        Sskip)
+      (Ssequence
+        (Ssequence
+          (Ssequence
+            (Ssequence
+              (Sset _t'5
+                (Ederef (Etempvar _sptr (tptr (tptr tvoid))) (tptr tvoid)))
+              (Sset _t'3 (Ecast (Etempvar _t'5 (tptr tvoid)) (tptr tint))))
+            (Sset _st (Etempvar _t'3 (tptr tint))))
+          (Sifthenelse (Eunop Onotbool (Etempvar _t'3 (tptr tint)) tint)
+            (Ssequence
+              (Ssequence
+                (Ssequence
+                  (Ssequence
+                    (Scall (Some _t'1)
+                      (Evar _calloc (Tfunction
+                                      (Tcons tuint (Tcons tuint Tnil))
+                                      (tptr tvoid) cc_default))
+                      ((Econst_int (Int.repr 1) tint) ::
+                       (Esizeof tint tuint) :: nil))
+                    (Sset _t'2
+                      (Ecast (Etempvar _t'1 (tptr tvoid)) (tptr tvoid))))
+                  (Sassign
+                    (Ederef (Etempvar _sptr (tptr (tptr tvoid)))
+                      (tptr tvoid)) (Etempvar _t'2 (tptr tvoid))))
+                (Sset _st (Ecast (Etempvar _t'2 (tptr tvoid)) (tptr tint))))
+              (Sifthenelse (Eunop Onotbool (Etempvar _st (tptr tint)) tint)
+                (Sloop
+                  (Ssequence
+                    (Sassign
+                      (Efield
+                        (Evar _tmp_error__1 (Tstruct _asn_dec_rval_s noattr))
+                        _code tint) (Econst_int (Int.repr 2) tint))
+                    (Ssequence
+                      (Sassign
+                        (Efield
+                          (Evar _tmp_error__1 (Tstruct _asn_dec_rval_s noattr))
+                          _consumed tuint) (Econst_int (Int.repr 0) tint))
+                      (Ssequence
+                        (Sloop Sskip Sbreak)
+                        (Ssequence
+                          (Sassign
+                            (Ederef
+                              (Etempvar __res (tptr (Tstruct _asn_dec_rval_s noattr)))
+                              (Tstruct _asn_dec_rval_s noattr))
+                            (Evar _tmp_error__1 (Tstruct _asn_dec_rval_s noattr)))
+                          (Sreturn None)))))
+                  Sbreak)
+                Sskip))
+            Sskip))
+        (Ssequence
+          (Ssequence
+            (Sset _t'4
+              (Ederef (Ecast (Etempvar _ptr (tptr tvoid)) (tptr tuchar))
+                tuchar))
+            (Sassign (Ederef (Etempvar _st (tptr tint)) tint)
+              (Etempvar _t'4 tuchar)))
+          (Ssequence
+            (Sassign
+              (Ederef
+                (Etempvar __res (tptr (Tstruct _asn_dec_rval_s noattr)))
+                (Tstruct _asn_dec_rval_s noattr))
+              (Evar _ok (Tstruct _asn_dec_rval_s noattr)))
+            (Sreturn None)))))))
+|}.
+
+Definition f_BOOLEAN_compare := {|
+  fn_return := tint;
+  fn_callconv := cc_default;
+  fn_params := ((_td, (tptr (Tstruct _asn_TYPE_descriptor_s noattr))) ::
+                (_aptr, (tptr tvoid)) :: (_bptr, (tptr tvoid)) :: nil);
+  fn_vars := nil;
+  fn_temps := ((_a, (tptr tint)) :: (_b, (tptr tint)) :: (_t'1, tint) ::
+               (_t'4, tint) :: (_t'3, tint) :: (_t'2, tint) :: nil);
+  fn_body :=
+(Ssequence
+  (Sset _a (Etempvar _aptr (tptr tvoid)))
+  (Ssequence
+    (Sset _b (Etempvar _bptr (tptr tvoid)))
+    (Ssequence
+      (Sifthenelse (Etempvar _a (tptr tint))
+        (Sset _t'1 (Ecast (Etempvar _b (tptr tint)) tbool))
+        (Sset _t'1 (Econst_int (Int.repr 0) tint)))
+      (Sifthenelse (Etempvar _t'1 tint)
+        (Ssequence
+          (Sset _t'2 (Ederef (Etempvar _a (tptr tint)) tint))
+          (Ssequence
+            (Sset _t'3 (Ederef (Etempvar _b (tptr tint)) tint))
+            (Sifthenelse (Ebinop Oeq
+                           (Eunop Onotbool (Etempvar _t'2 tint) tint)
+                           (Eunop Onotbool (Etempvar _t'3 tint) tint) tint)
+              (Sreturn (Some (Econst_int (Int.repr 0) tint)))
+              (Ssequence
+                (Sset _t'4 (Ederef (Etempvar _a (tptr tint)) tint))
+                (Sifthenelse (Eunop Onotbool (Etempvar _t'4 tint) tint)
+                  (Sreturn (Some (Eunop Oneg (Econst_int (Int.repr 1) tint)
+                                   tint)))
+                  (Sreturn (Some (Econst_int (Int.repr 1) tint))))))))
+        (Sifthenelse (Eunop Onotbool (Etempvar _a (tptr tint)) tint)
+          (Sreturn (Some (Eunop Oneg (Econst_int (Int.repr 1) tint) tint)))
+          (Sreturn (Some (Econst_int (Int.repr 1) tint))))))))
+|}.
+
+Definition f_BOOLEAN_random_fill := {|
+  fn_return := tvoid;
+  fn_callconv := {|cc_vararg:=false; cc_unproto:=false; cc_structret:=true|};
+  fn_params := ((__res, (tptr (Tstruct _asn_random_fill_result_s noattr))) ::
+                (_td, (tptr (Tstruct _asn_TYPE_descriptor_s noattr))) ::
+                (_sptr, (tptr (tptr tvoid))) ::
+                (_constraints,
+                 (tptr (Tstruct _asn_encoding_constraints_s noattr))) ::
+                (_max_length, tuint) :: nil);
+  fn_vars := ((_result_ok, (Tstruct _asn_random_fill_result_s noattr)) ::
+              (_result_failed, (Tstruct _asn_random_fill_result_s noattr)) ::
+              (_result_skipped, (Tstruct _asn_random_fill_result_s noattr)) ::
+              nil);
+  fn_temps := ((_st, (tptr tint)) ::
+               (_pc, (tptr (Tstruct _asn_per_constraint_s noattr))) ::
+               (_t'6, tlong) :: (_t'5, tlong) :: (_t'4, tlong) ::
+               (_t'3, tint) :: (_t'2, (tptr tvoid)) ::
+               (_t'1, (tptr tvoid)) ::
+               (_t'12, (tptr (Tstruct _asn_per_constraints_s noattr))) ::
+               (_t'11, (tptr (Tstruct _asn_per_constraints_s noattr))) ::
+               (_t'10, tint) :: (_t'9, tint) :: (_t'8, tint) ::
+               (_t'7, (tptr (Tstruct _asn_per_constraints_s noattr))) :: nil);
+  fn_body :=
+(Ssequence
+  (Sassign
+    (Efield (Evar _result_ok (Tstruct _asn_random_fill_result_s noattr))
+      _code tint) (Econst_int (Int.repr 0) tint))
+  (Ssequence
+    (Sassign
+      (Efield (Evar _result_ok (Tstruct _asn_random_fill_result_s noattr))
+        _length tuint) (Econst_int (Int.repr 1) tint))
+    (Ssequence
+      (Sassign
+        (Efield
+          (Evar _result_failed (Tstruct _asn_random_fill_result_s noattr))
+          _code tint) (Econst_int (Int.repr (-1)) tint))
+      (Ssequence
+        (Sassign
+          (Efield
+            (Evar _result_failed (Tstruct _asn_random_fill_result_s noattr))
+            _length tuint) (Econst_int (Int.repr 0) tint))
+        (Ssequence
+          (Sassign
+            (Efield
+              (Evar _result_skipped (Tstruct _asn_random_fill_result_s noattr))
+              _code tint) (Econst_int (Int.repr 1) tint))
+          (Ssequence
+            (Sassign
+              (Efield
+                (Evar _result_skipped (Tstruct _asn_random_fill_result_s noattr))
+                _length tuint) (Econst_int (Int.repr 0) tint))
+            (Ssequence
+              (Sset _st
+                (Ederef (Etempvar _sptr (tptr (tptr tvoid))) (tptr tvoid)))
+              (Ssequence
+                (Sifthenelse (Ebinop Oeq (Etempvar _max_length tuint)
+                               (Econst_int (Int.repr 0) tint) tint)
+                  (Ssequence
+                    (Sassign
+                      (Ederef
+                        (Etempvar __res (tptr (Tstruct _asn_random_fill_result_s noattr)))
+                        (Tstruct _asn_random_fill_result_s noattr))
+                      (Evar _result_skipped (Tstruct _asn_random_fill_result_s noattr)))
+                    (Sreturn None))
+                  Sskip)
+                (Ssequence
+                  (Sifthenelse (Ebinop Oeq (Etempvar _st (tptr tint))
+                                 (Ecast (Econst_int (Int.repr 0) tint)
+                                   (tptr tvoid)) tint)
+                    (Ssequence
+                      (Ssequence
+                        (Ssequence
+                          (Ssequence
+                            (Scall (Some _t'1)
+                              (Evar _calloc (Tfunction
+                                              (Tcons tuint
+                                                (Tcons tuint Tnil))
+                                              (tptr tvoid) cc_default))
+                              ((Econst_int (Int.repr 1) tint) ::
+                               (Esizeof tint tuint) :: nil))
+                            (Sset _t'2
+                              (Ecast (Etempvar _t'1 (tptr tvoid))
+                                (tptr tvoid))))
+                          (Sassign
+                            (Ederef (Etempvar _sptr (tptr (tptr tvoid)))
+                              (tptr tvoid)) (Etempvar _t'2 (tptr tvoid))))
+                        (Sset _st
+                          (Ecast (Etempvar _t'2 (tptr tvoid)) (tptr tint))))
+                      (Sifthenelse (Ebinop Oeq (Etempvar _st (tptr tint))
+                                     (Ecast (Econst_int (Int.repr 0) tint)
+                                       (tptr tvoid)) tint)
+                        (Ssequence
+                          (Sassign
+                            (Ederef
+                              (Etempvar __res (tptr (Tstruct _asn_random_fill_result_s noattr)))
+                              (Tstruct _asn_random_fill_result_s noattr))
+                            (Evar _result_failed (Tstruct _asn_random_fill_result_s noattr)))
+                          (Sreturn None))
+                        Sskip))
+                    Sskip)
+                  (Ssequence
+                    (Ssequence
+                      (Sifthenelse (Eunop Onotbool
+                                     (Etempvar _constraints (tptr (Tstruct _asn_encoding_constraints_s noattr)))
+                                     tint)
+                        (Sset _t'3 (Econst_int (Int.repr 1) tint))
+                        (Ssequence
+                          (Sset _t'12
+                            (Efield
+                              (Ederef
+                                (Etempvar _constraints (tptr (Tstruct _asn_encoding_constraints_s noattr)))
+                                (Tstruct _asn_encoding_constraints_s noattr))
+                              _per_constraints
+                              (tptr (Tstruct _asn_per_constraints_s noattr))))
+                          (Sset _t'3
+                            (Ecast
+                              (Eunop Onotbool
+                                (Etempvar _t'12 (tptr (Tstruct _asn_per_constraints_s noattr)))
+                                tint) tbool))))
+                      (Sifthenelse (Etempvar _t'3 tint)
+                        (Sset _constraints
+                          (Eaddrof
+                            (Efield
+                              (Ederef
+                                (Etempvar _td (tptr (Tstruct _asn_TYPE_descriptor_s noattr)))
+                                (Tstruct _asn_TYPE_descriptor_s noattr))
+                              _encoding_constraints
+                              (Tstruct _asn_encoding_constraints_s noattr))
+                            (tptr (Tstruct _asn_encoding_constraints_s noattr))))
+                        Sskip))
+                    (Ssequence
+                      (Ssequence
+                        (Sset _t'7
+                          (Efield
+                            (Ederef
+                              (Etempvar _constraints (tptr (Tstruct _asn_encoding_constraints_s noattr)))
+                              (Tstruct _asn_encoding_constraints_s noattr))
+                            _per_constraints
+                            (tptr (Tstruct _asn_per_constraints_s noattr))))
+                        (Sifthenelse (Etempvar _t'7 (tptr (Tstruct _asn_per_constraints_s noattr)))
+                          (Ssequence
+                            (Ssequence
+                              (Sset _t'11
+                                (Efield
+                                  (Ederef
+                                    (Etempvar _constraints (tptr (Tstruct _asn_encoding_constraints_s noattr)))
+                                    (Tstruct _asn_encoding_constraints_s noattr))
+                                  _per_constraints
+                                  (tptr (Tstruct _asn_per_constraints_s noattr))))
+                              (Sset _pc
+                                (Eaddrof
+                                  (Efield
+                                    (Ederef
+                                      (Etempvar _t'11 (tptr (Tstruct _asn_per_constraints_s noattr)))
+                                      (Tstruct _asn_per_constraints_s noattr))
+                                    _value
+                                    (Tstruct _asn_per_constraint_s noattr))
+                                  (tptr (Tstruct _asn_per_constraint_s noattr)))))
+                            (Ssequence
+                              (Sset _t'8
+                                (Efield
+                                  (Ederef
+                                    (Etempvar _pc (tptr (Tstruct _asn_per_constraint_s noattr)))
+                                    (Tstruct _asn_per_constraint_s noattr))
+                                  _flags tint))
+                              (Sifthenelse (Ebinop Oand (Etempvar _t'8 tint)
+                                             (Econst_int (Int.repr 2) tint)
+                                             tint)
+                                (Ssequence
+                                  (Ssequence
+                                    (Ssequence
+                                      (Sset _t'9
+                                        (Efield
+                                          (Ederef
+                                            (Etempvar _pc (tptr (Tstruct _asn_per_constraint_s noattr)))
+                                            (Tstruct _asn_per_constraint_s noattr))
+                                          _lower_bound tint))
+                                      (Ssequence
+                                        (Sset _t'10
+                                          (Efield
+                                            (Ederef
+                                              (Etempvar _pc (tptr (Tstruct _asn_per_constraint_s noattr)))
+                                              (Tstruct _asn_per_constraint_s noattr))
+                                            _upper_bound tint))
+                                        (Scall (Some _t'4)
+                                          (Evar _asn_random_between (Tfunction
+                                                                    (Tcons
+                                                                    tlong
+                                                                    (Tcons
+                                                                    tlong
+                                                                    Tnil))
+                                                                    tlong
+                                                                    cc_default))
+                                          ((Etempvar _t'9 tint) ::
+                                           (Etempvar _t'10 tint) :: nil))))
+                                    (Sassign
+                                      (Ederef (Etempvar _st (tptr tint))
+                                        tint) (Etempvar _t'4 tlong)))
+                                  (Ssequence
+                                    (Sassign
+                                      (Ederef
+                                        (Etempvar __res (tptr (Tstruct _asn_random_fill_result_s noattr)))
+                                        (Tstruct _asn_random_fill_result_s noattr))
+                                      (Evar _result_ok (Tstruct _asn_random_fill_result_s noattr)))
+                                    (Sreturn None)))
+                                Sskip)))
+                          Sskip))
+                      (Ssequence
+                        (Ssequence
+                          (Scall (Some _t'5)
+                            (Evar _asn_random_between (Tfunction
+                                                        (Tcons tlong
+                                                          (Tcons tlong Tnil))
+                                                        tlong cc_default))
+                            ((Econst_int (Int.repr 0) tint) ::
+                             (Econst_int (Int.repr 7) tint) :: nil))
+                          (Sswitch (Etempvar _t'5 tlong)
+                            (LScons (Some 0)
+                              Sskip
+                              (LScons (Some 1)
+                                Sskip
+                                (LScons (Some 2)
+                                  (Ssequence
+                                    (Sassign
+                                      (Ederef (Etempvar _st (tptr tint))
+                                        tint) (Econst_int (Int.repr 0) tint))
+                                    Sbreak)
+                                  (LScons (Some 3)
+                                    (Ssequence
+                                      (Sassign
+                                        (Ederef (Etempvar _st (tptr tint))
+                                          tint)
+                                        (Eunop Oneg
+                                          (Econst_int (Int.repr 1) tint)
+                                          tint))
+                                      Sbreak)
+                                    (LScons (Some 4)
+                                      (Ssequence
+                                        (Sassign
+                                          (Ederef (Etempvar _st (tptr tint))
+                                            tint)
+                                          (Econst_int (Int.repr 1) tint))
+                                        Sbreak)
+                                      (LScons (Some 5)
+                                        (Ssequence
+                                          (Sassign
+                                            (Ederef
+                                              (Etempvar _st (tptr tint))
+                                              tint)
+                                            (Ebinop Osub
+                                              (Eunop Oneg
+                                                (Econst_int (Int.repr 2147483647) tint)
+                                                tint)
+                                              (Econst_int (Int.repr 1) tint)
+                                              tint))
+                                          Sbreak)
+                                        (LScons (Some 6)
+                                          (Ssequence
+                                            (Sassign
+                                              (Ederef
+                                                (Etempvar _st (tptr tint))
+                                                tint)
+                                              (Econst_int (Int.repr 2147483647) tint))
+                                            Sbreak)
+                                          (LScons None
+                                            (Ssequence
+                                              (Ssequence
+                                                (Scall (Some _t'6)
+                                                  (Evar _asn_random_between 
+                                                  (Tfunction
+                                                    (Tcons tlong
+                                                      (Tcons tlong Tnil))
+                                                    tlong cc_default))
+                                                  ((Ebinop Osub
+                                                     (Eunop Oneg
+                                                       (Econst_int (Int.repr 2147483647) tint)
+                                                       tint)
+                                                     (Econst_int (Int.repr 1) tint)
+                                                     tint) ::
+                                                   (Econst_int (Int.repr 2147483647) tint) ::
+                                                   nil))
+                                                (Sassign
+                                                  (Ederef
+                                                    (Etempvar _st (tptr tint))
+                                                    tint)
+                                                  (Etempvar _t'6 tlong)))
+                                              Sbreak)
+                                            LSnil))))))))))
+                        (Ssequence
+                          (Sassign
+                            (Ederef
+                              (Etempvar __res (tptr (Tstruct _asn_random_fill_result_s noattr)))
+                              (Tstruct _asn_random_fill_result_s noattr))
+                            (Evar _result_ok (Tstruct _asn_random_fill_result_s noattr)))
+                          (Sreturn None))))))))))))))
+|}.
+
+Definition composites : list composite_definition :=
+(Composite _asn_codec_ctx_s Struct ((_max_stack_size, tuint) :: nil) noattr ::
+ Composite _asn_enc_rval_s Struct
+   ((_encoded, tint) ::
+    (_failed_type, (tptr (Tstruct _asn_TYPE_descriptor_s noattr))) ::
+    (_structure_ptr, (tptr tvoid)) :: nil)
+   noattr ::
+ Composite _asn_dec_rval_s Struct
+   ((_code, tint) :: (_consumed, tuint) :: nil)
+   noattr ::
+ Composite _asn_struct_ctx_s Struct
+   ((_phase, tshort) :: (_step, tshort) :: (_context, tint) ::
+    (_ptr, (tptr tvoid)) :: (_left, tint) :: nil)
+   noattr ::
+ Composite _asn_bit_data_s Struct
+   ((_buffer, (tptr tuchar)) :: (_nboff, tuint) :: (_nbits, tuint) ::
+    (_moved, tuint) ::
+    (_refill,
+     (tptr (Tfunction (Tcons (tptr (Tstruct _asn_bit_data_s noattr)) Tnil)
+             tint cc_default))) :: (_refill_key, (tptr tvoid)) :: nil)
+   noattr ::
+ Composite _asn_bit_outp_s Struct
+   ((_buffer, (tptr tuchar)) :: (_nboff, tuint) :: (_nbits, tuint) ::
+    (_tmpspace, (tarray tuchar 32)) ::
+    (_output,
+     (tptr (Tfunction
+             (Tcons (tptr tvoid) (Tcons tuint (Tcons (tptr tvoid) Tnil)))
+             tint cc_default))) :: (_op_key, (tptr tvoid)) ::
+    (_flushed_bytes, tuint) :: nil)
+   noattr ::
+ Composite _asn_per_constraint_s Struct
+   ((_flags, tint) :: (_range_bits, tint) :: (_effective_bits, tint) ::
+    (_lower_bound, tint) :: (_upper_bound, tint) :: nil)
+   noattr ::
+ Composite _asn_per_constraints_s Struct
+   ((_value, (Tstruct _asn_per_constraint_s noattr)) ::
+    (_size, (Tstruct _asn_per_constraint_s noattr)) ::
+    (_value2code, (tptr (Tfunction (Tcons tuint Tnil) tint cc_default))) ::
+    (_code2value, (tptr (Tfunction (Tcons tuint Tnil) tint cc_default))) ::
+    nil)
+   noattr ::
+ Composite _asn_random_fill_result_s Struct
+   ((_code, tint) :: (_length, tuint) :: nil)
+   noattr ::
+ Composite _asn_oer_constraint_number_s Struct
+   ((_width, tuint) :: (_positive, tuint) :: nil)
+   noattr ::
+ Composite _asn_oer_constraints_s Struct
+   ((_value, (Tstruct _asn_oer_constraint_number_s noattr)) ::
+    (_size, tint) :: nil)
+   noattr ::
+ Composite _asn_type_selector_result_s Struct
+   ((_type_descriptor, (tptr (Tstruct _asn_TYPE_descriptor_s noattr))) ::
+    (_presence_index, tuint) :: nil)
+   noattr ::
+ Composite _asn_TYPE_operation_s Struct
+   ((_free_struct,
+     (tptr (Tfunction
+             (Tcons (tptr (Tstruct _asn_TYPE_descriptor_s noattr))
+               (Tcons (tptr tvoid) (Tcons tint Tnil))) tvoid cc_default))) ::
+    (_print_struct,
+     (tptr (Tfunction
+             (Tcons (tptr (Tstruct _asn_TYPE_descriptor_s noattr))
+               (Tcons (tptr tvoid)
+                 (Tcons tint
+                   (Tcons
+                     (tptr (Tfunction
+                             (Tcons (tptr tvoid)
+                               (Tcons tuint (Tcons (tptr tvoid) Tnil))) tint
+                             cc_default)) (Tcons (tptr tvoid) Tnil))))) tint
+             cc_default))) ::
+    (_compare_struct,
+     (tptr (Tfunction
+             (Tcons (tptr (Tstruct _asn_TYPE_descriptor_s noattr))
+               (Tcons (tptr tvoid) (Tcons (tptr tvoid) Tnil))) tint
+             cc_default))) ::
+    (_ber_decoder,
+     (tptr (Tfunction
+             (Tcons (tptr (Tstruct _asn_dec_rval_s noattr))
+               (Tcons (tptr (Tstruct _asn_codec_ctx_s noattr))
+                 (Tcons (tptr (Tstruct _asn_TYPE_descriptor_s noattr))
+                   (Tcons (tptr (tptr tvoid))
+                     (Tcons (tptr tvoid) (Tcons tuint (Tcons tint Tnil)))))))
+             tvoid
+             {|cc_vararg:=false; cc_unproto:=false; cc_structret:=true|}))) ::
+    (_der_encoder,
+     (tptr (Tfunction
+             (Tcons (tptr (Tstruct _asn_enc_rval_s noattr))
+               (Tcons (tptr (Tstruct _asn_TYPE_descriptor_s noattr))
+                 (Tcons (tptr tvoid)
+                   (Tcons tint
+                     (Tcons tuint
+                       (Tcons
+                         (tptr (Tfunction
+                                 (Tcons (tptr tvoid)
+                                   (Tcons tuint (Tcons (tptr tvoid) Tnil)))
+                                 tint cc_default)) (Tcons (tptr tvoid) Tnil)))))))
+             tvoid
+             {|cc_vararg:=false; cc_unproto:=false; cc_structret:=true|}))) ::
+    (_xer_decoder,
+     (tptr (Tfunction
+             (Tcons (tptr (Tstruct _asn_dec_rval_s noattr))
+               (Tcons (tptr (Tstruct _asn_codec_ctx_s noattr))
+                 (Tcons (tptr (Tstruct _asn_TYPE_descriptor_s noattr))
+                   (Tcons (tptr (tptr tvoid))
+                     (Tcons (tptr tschar)
+                       (Tcons (tptr tvoid) (Tcons tuint Tnil))))))) tvoid
+             {|cc_vararg:=false; cc_unproto:=false; cc_structret:=true|}))) ::
+    (_xer_encoder,
+     (tptr (Tfunction
+             (Tcons (tptr (Tstruct _asn_enc_rval_s noattr))
+               (Tcons (tptr (Tstruct _asn_TYPE_descriptor_s noattr))
+                 (Tcons (tptr tvoid)
+                   (Tcons tint
+                     (Tcons tint
+                       (Tcons
+                         (tptr (Tfunction
+                                 (Tcons (tptr tvoid)
+                                   (Tcons tuint (Tcons (tptr tvoid) Tnil)))
+                                 tint cc_default)) (Tcons (tptr tvoid) Tnil)))))))
+             tvoid
+             {|cc_vararg:=false; cc_unproto:=false; cc_structret:=true|}))) ::
+    (_oer_decoder,
+     (tptr (Tfunction
+             (Tcons (tptr (Tstruct _asn_dec_rval_s noattr))
+               (Tcons (tptr (Tstruct _asn_codec_ctx_s noattr))
+                 (Tcons (tptr (Tstruct _asn_TYPE_descriptor_s noattr))
+                   (Tcons (tptr (Tstruct _asn_oer_constraints_s noattr))
+                     (Tcons (tptr (tptr tvoid))
+                       (Tcons (tptr tvoid) (Tcons tuint Tnil))))))) tvoid
+             {|cc_vararg:=false; cc_unproto:=false; cc_structret:=true|}))) ::
+    (_oer_encoder,
+     (tptr (Tfunction
+             (Tcons (tptr (Tstruct _asn_enc_rval_s noattr))
+               (Tcons (tptr (Tstruct _asn_TYPE_descriptor_s noattr))
+                 (Tcons (tptr (Tstruct _asn_oer_constraints_s noattr))
+                   (Tcons (tptr tvoid)
+                     (Tcons
+                       (tptr (Tfunction
+                               (Tcons (tptr tvoid)
+                                 (Tcons tuint (Tcons (tptr tvoid) Tnil)))
+                               tint cc_default)) (Tcons (tptr tvoid) Tnil))))))
+             tvoid
+             {|cc_vararg:=false; cc_unproto:=false; cc_structret:=true|}))) ::
+    (_uper_decoder,
+     (tptr (Tfunction
+             (Tcons (tptr (Tstruct _asn_dec_rval_s noattr))
+               (Tcons (tptr (Tstruct _asn_codec_ctx_s noattr))
+                 (Tcons (tptr (Tstruct _asn_TYPE_descriptor_s noattr))
+                   (Tcons (tptr (Tstruct _asn_per_constraints_s noattr))
+                     (Tcons (tptr (tptr tvoid))
+                       (Tcons (tptr (Tstruct _asn_bit_data_s noattr)) Tnil))))))
+             tvoid
+             {|cc_vararg:=false; cc_unproto:=false; cc_structret:=true|}))) ::
+    (_uper_encoder,
+     (tptr (Tfunction
+             (Tcons (tptr (Tstruct _asn_enc_rval_s noattr))
+               (Tcons (tptr (Tstruct _asn_TYPE_descriptor_s noattr))
+                 (Tcons (tptr (Tstruct _asn_per_constraints_s noattr))
+                   (Tcons (tptr tvoid)
+                     (Tcons (tptr (Tstruct _asn_bit_outp_s noattr)) Tnil)))))
+             tvoid
+             {|cc_vararg:=false; cc_unproto:=false; cc_structret:=true|}))) ::
+    (_random_fill,
+     (tptr (Tfunction
+             (Tcons (tptr (Tstruct _asn_random_fill_result_s noattr))
+               (Tcons (tptr (Tstruct _asn_TYPE_descriptor_s noattr))
+                 (Tcons (tptr (tptr tvoid))
+                   (Tcons (tptr (Tstruct _asn_encoding_constraints_s noattr))
+                     (Tcons tuint Tnil))))) tvoid
+             {|cc_vararg:=false; cc_unproto:=false; cc_structret:=true|}))) ::
+    (_outmost_tag,
+     (tptr (Tfunction
+             (Tcons (tptr (Tstruct _asn_TYPE_descriptor_s noattr))
+               (Tcons (tptr tvoid) (Tcons tint (Tcons tuint Tnil)))) tuint
+             cc_default))) :: nil)
+   noattr ::
+ Composite _asn_encoding_constraints_s Struct
+   ((_oer_constraints, (tptr (Tstruct _asn_oer_constraints_s noattr))) ::
+    (_per_constraints, (tptr (Tstruct _asn_per_constraints_s noattr))) ::
+    (_general_constraints,
+     (tptr (Tfunction
+             (Tcons (tptr (Tstruct _asn_TYPE_descriptor_s noattr))
+               (Tcons (tptr tvoid)
+                 (Tcons
+                   (tptr (Tfunction
+                           (Tcons (tptr tvoid)
+                             (Tcons
+                               (tptr (Tstruct _asn_TYPE_descriptor_s noattr))
+                               (Tcons (tptr tvoid)
+                                 (Tcons (tptr tschar) Tnil)))) tvoid
+                           {|cc_vararg:=true; cc_unproto:=false; cc_structret:=false|}))
+                   (Tcons (tptr tvoid) Tnil)))) tint cc_default))) :: nil)
+   noattr ::
+ Composite _asn_TYPE_descriptor_s Struct
+   ((_name, (tptr tschar)) :: (_xml_tag, (tptr tschar)) ::
+    (_op, (tptr (Tstruct _asn_TYPE_operation_s noattr))) ::
+    (_tags, (tptr tuint)) :: (_tags_count, tuint) ::
+    (_all_tags, (tptr tuint)) :: (_all_tags_count, tuint) ::
+    (_encoding_constraints, (Tstruct _asn_encoding_constraints_s noattr)) ::
+    (_elements, (tptr (Tstruct _asn_TYPE_member_s noattr))) ::
+    (_elements_count, tuint) :: (_specifics, (tptr tvoid)) :: nil)
+   noattr ::
+ Composite _asn_TYPE_member_s Struct
+   ((_flags, tint) :: (_optional, tuint) :: (_memb_offset, tuint) ::
+    (_tag, tuint) :: (_tag_mode, tint) ::
+    (_type, (tptr (Tstruct _asn_TYPE_descriptor_s noattr))) ::
+    (_type_selector,
+     (tptr (Tfunction
+             (Tcons (tptr (Tstruct _asn_type_selector_result_s noattr))
+               (Tcons (tptr (Tstruct _asn_TYPE_descriptor_s noattr))
+                 (Tcons (tptr tvoid) Tnil))) tvoid
+             {|cc_vararg:=false; cc_unproto:=false; cc_structret:=true|}))) ::
+    (_encoding_constraints, (Tstruct _asn_encoding_constraints_s noattr)) ::
+    (_default_value_cmp,
+     (tptr (Tfunction (Tcons (tptr tvoid) Tnil) tint cc_default))) ::
+    (_default_value_set,
+     (tptr (Tfunction (Tcons (tptr (tptr tvoid)) Tnil) tint cc_default))) ::
+    (_name, (tptr tschar)) :: nil)
+   noattr :: nil).
+
+Definition global_definitions : list (ident * globdef fundef type) :=
+((___stringlit_1, Gvar v___stringlit_1) ::
+ (___stringlit_3, Gvar v___stringlit_3) ::
+ (___stringlit_4, Gvar v___stringlit_4) ::
+ (___stringlit_7, Gvar v___stringlit_7) ::
+ (___stringlit_8, Gvar v___stringlit_8) ::
+ (___stringlit_5, Gvar v___stringlit_5) ::
+ (___stringlit_2, Gvar v___stringlit_2) ::
+ (___stringlit_6, Gvar v___stringlit_6) ::
+ (___builtin_ais_annot,
+   Gfun(External (EF_builtin "__builtin_ais_annot"
+                   (mksignature (AST.Tint :: nil) None
+                     {|cc_vararg:=true; cc_unproto:=false; cc_structret:=false|}))
+     (Tcons (tptr tschar) Tnil) tvoid
+     {|cc_vararg:=true; cc_unproto:=false; cc_structret:=false|})) ::
+ (___builtin_bswap,
+   Gfun(External (EF_builtin "__builtin_bswap"
+                   (mksignature (AST.Tint :: nil) (Some AST.Tint) cc_default))
+     (Tcons tuint Tnil) tuint cc_default)) ::
+ (___builtin_bswap32,
+   Gfun(External (EF_builtin "__builtin_bswap32"
+                   (mksignature (AST.Tint :: nil) (Some AST.Tint) cc_default))
+     (Tcons tuint Tnil) tuint cc_default)) ::
+ (___builtin_bswap16,
+   Gfun(External (EF_builtin "__builtin_bswap16"
+                   (mksignature (AST.Tint :: nil) (Some AST.Tint) cc_default))
+     (Tcons tushort Tnil) tushort cc_default)) ::
+ (___builtin_fabs,
+   Gfun(External (EF_builtin "__builtin_fabs"
+                   (mksignature (AST.Tfloat :: nil) (Some AST.Tfloat)
+                     cc_default)) (Tcons tdouble Tnil) tdouble cc_default)) ::
+ (___builtin_fsqrt,
+   Gfun(External (EF_builtin "__builtin_fsqrt"
+                   (mksignature (AST.Tfloat :: nil) (Some AST.Tfloat)
+                     cc_default)) (Tcons tdouble Tnil) tdouble cc_default)) ::
+ (___builtin_memcpy_aligned,
+   Gfun(External (EF_builtin "__builtin_memcpy_aligned"
+                   (mksignature
+                     (AST.Tint :: AST.Tint :: AST.Tint :: AST.Tint :: nil)
+                     None cc_default))
+     (Tcons (tptr tvoid)
+       (Tcons (tptr tvoid) (Tcons tuint (Tcons tuint Tnil)))) tvoid
+     cc_default)) ::
+ (___builtin_annot,
+   Gfun(External (EF_builtin "__builtin_annot"
+                   (mksignature (AST.Tint :: nil) None
+                     {|cc_vararg:=true; cc_unproto:=false; cc_structret:=false|}))
+     (Tcons (tptr tschar) Tnil) tvoid
+     {|cc_vararg:=true; cc_unproto:=false; cc_structret:=false|})) ::
+ (___builtin_annot_intval,
+   Gfun(External (EF_builtin "__builtin_annot_intval"
+                   (mksignature (AST.Tint :: AST.Tint :: nil) (Some AST.Tint)
+                     cc_default)) (Tcons (tptr tschar) (Tcons tint Tnil))
+     tint cc_default)) ::
+ (___builtin_membar,
+   Gfun(External (EF_builtin "__builtin_membar"
+                   (mksignature nil None cc_default)) Tnil tvoid cc_default)) ::
+ (___builtin_va_start,
+   Gfun(External (EF_builtin "__builtin_va_start"
+                   (mksignature (AST.Tint :: nil) None cc_default))
+     (Tcons (tptr tvoid) Tnil) tvoid cc_default)) ::
+ (___builtin_va_arg,
+   Gfun(External (EF_builtin "__builtin_va_arg"
+                   (mksignature (AST.Tint :: AST.Tint :: nil) None
+                     cc_default)) (Tcons (tptr tvoid) (Tcons tuint Tnil))
+     tvoid cc_default)) ::
+ (___builtin_va_copy,
+   Gfun(External (EF_builtin "__builtin_va_copy"
+                   (mksignature (AST.Tint :: AST.Tint :: nil) None
+                     cc_default))
+     (Tcons (tptr tvoid) (Tcons (tptr tvoid) Tnil)) tvoid cc_default)) ::
+ (___builtin_va_end,
+   Gfun(External (EF_builtin "__builtin_va_end"
+                   (mksignature (AST.Tint :: nil) None cc_default))
+     (Tcons (tptr tvoid) Tnil) tvoid cc_default)) ::
+ (___compcert_va_int32,
+   Gfun(External (EF_external "__compcert_va_int32"
+                   (mksignature (AST.Tint :: nil) (Some AST.Tint) cc_default))
+     (Tcons (tptr tvoid) Tnil) tuint cc_default)) ::
+ (___compcert_va_int64,
+   Gfun(External (EF_external "__compcert_va_int64"
+                   (mksignature (AST.Tint :: nil) (Some AST.Tlong)
+                     cc_default)) (Tcons (tptr tvoid) Tnil) tulong
+     cc_default)) ::
+ (___compcert_va_float64,
+   Gfun(External (EF_external "__compcert_va_float64"
+                   (mksignature (AST.Tint :: nil) (Some AST.Tfloat)
+                     cc_default)) (Tcons (tptr tvoid) Tnil) tdouble
+     cc_default)) ::
+ (___compcert_va_composite,
+   Gfun(External (EF_external "__compcert_va_composite"
+                   (mksignature (AST.Tint :: AST.Tint :: nil) (Some AST.Tint)
+                     cc_default)) (Tcons (tptr tvoid) (Tcons tuint Tnil))
+     (tptr tvoid) cc_default)) ::
+ (___compcert_i64_dtos,
+   Gfun(External (EF_runtime "__compcert_i64_dtos"
+                   (mksignature (AST.Tfloat :: nil) (Some AST.Tlong)
+                     cc_default)) (Tcons tdouble Tnil) tlong cc_default)) ::
+ (___compcert_i64_dtou,
+   Gfun(External (EF_runtime "__compcert_i64_dtou"
+                   (mksignature (AST.Tfloat :: nil) (Some AST.Tlong)
+                     cc_default)) (Tcons tdouble Tnil) tulong cc_default)) ::
+ (___compcert_i64_stod,
+   Gfun(External (EF_runtime "__compcert_i64_stod"
+                   (mksignature (AST.Tlong :: nil) (Some AST.Tfloat)
+                     cc_default)) (Tcons tlong Tnil) tdouble cc_default)) ::
+ (___compcert_i64_utod,
+   Gfun(External (EF_runtime "__compcert_i64_utod"
+                   (mksignature (AST.Tlong :: nil) (Some AST.Tfloat)
+                     cc_default)) (Tcons tulong Tnil) tdouble cc_default)) ::
+ (___compcert_i64_stof,
+   Gfun(External (EF_runtime "__compcert_i64_stof"
+                   (mksignature (AST.Tlong :: nil) (Some AST.Tsingle)
+                     cc_default)) (Tcons tlong Tnil) tfloat cc_default)) ::
+ (___compcert_i64_utof,
+   Gfun(External (EF_runtime "__compcert_i64_utof"
+                   (mksignature (AST.Tlong :: nil) (Some AST.Tsingle)
+                     cc_default)) (Tcons tulong Tnil) tfloat cc_default)) ::
+ (___compcert_i64_sdiv,
+   Gfun(External (EF_runtime "__compcert_i64_sdiv"
+                   (mksignature (AST.Tlong :: AST.Tlong :: nil)
+                     (Some AST.Tlong) cc_default))
+     (Tcons tlong (Tcons tlong Tnil)) tlong cc_default)) ::
+ (___compcert_i64_udiv,
+   Gfun(External (EF_runtime "__compcert_i64_udiv"
+                   (mksignature (AST.Tlong :: AST.Tlong :: nil)
+                     (Some AST.Tlong) cc_default))
+     (Tcons tulong (Tcons tulong Tnil)) tulong cc_default)) ::
+ (___compcert_i64_smod,
+   Gfun(External (EF_runtime "__compcert_i64_smod"
+                   (mksignature (AST.Tlong :: AST.Tlong :: nil)
+                     (Some AST.Tlong) cc_default))
+     (Tcons tlong (Tcons tlong Tnil)) tlong cc_default)) ::
+ (___compcert_i64_umod,
+   Gfun(External (EF_runtime "__compcert_i64_umod"
+                   (mksignature (AST.Tlong :: AST.Tlong :: nil)
+                     (Some AST.Tlong) cc_default))
+     (Tcons tulong (Tcons tulong Tnil)) tulong cc_default)) ::
+ (___compcert_i64_shl,
+   Gfun(External (EF_runtime "__compcert_i64_shl"
+                   (mksignature (AST.Tlong :: AST.Tint :: nil)
+                     (Some AST.Tlong) cc_default))
+     (Tcons tlong (Tcons tint Tnil)) tlong cc_default)) ::
+ (___compcert_i64_shr,
+   Gfun(External (EF_runtime "__compcert_i64_shr"
+                   (mksignature (AST.Tlong :: AST.Tint :: nil)
+                     (Some AST.Tlong) cc_default))
+     (Tcons tulong (Tcons tint Tnil)) tulong cc_default)) ::
+ (___compcert_i64_sar,
+   Gfun(External (EF_runtime "__compcert_i64_sar"
+                   (mksignature (AST.Tlong :: AST.Tint :: nil)
+                     (Some AST.Tlong) cc_default))
+     (Tcons tlong (Tcons tint Tnil)) tlong cc_default)) ::
+ (___compcert_i64_smulh,
+   Gfun(External (EF_runtime "__compcert_i64_smulh"
+                   (mksignature (AST.Tlong :: AST.Tlong :: nil)
+                     (Some AST.Tlong) cc_default))
+     (Tcons tlong (Tcons tlong Tnil)) tlong cc_default)) ::
+ (___compcert_i64_umulh,
+   Gfun(External (EF_runtime "__compcert_i64_umulh"
+                   (mksignature (AST.Tlong :: AST.Tlong :: nil)
+                     (Some AST.Tlong) cc_default))
+     (Tcons tulong (Tcons tulong Tnil)) tulong cc_default)) ::
+ (___builtin_bswap64,
+   Gfun(External (EF_builtin "__builtin_bswap64"
+                   (mksignature (AST.Tlong :: nil) (Some AST.Tlong)
+                     cc_default)) (Tcons tulong Tnil) tulong cc_default)) ::
+ (___builtin_clz,
+   Gfun(External (EF_builtin "__builtin_clz"
+                   (mksignature (AST.Tint :: nil) (Some AST.Tint) cc_default))
+     (Tcons tuint Tnil) tint cc_default)) ::
+ (___builtin_clzl,
+   Gfun(External (EF_builtin "__builtin_clzl"
+                   (mksignature (AST.Tint :: nil) (Some AST.Tint) cc_default))
+     (Tcons tuint Tnil) tint cc_default)) ::
+ (___builtin_clzll,
+   Gfun(External (EF_builtin "__builtin_clzll"
+                   (mksignature (AST.Tlong :: nil) (Some AST.Tint)
+                     cc_default)) (Tcons tulong Tnil) tint cc_default)) ::
+ (___builtin_ctz,
+   Gfun(External (EF_builtin "__builtin_ctz"
+                   (mksignature (AST.Tint :: nil) (Some AST.Tint) cc_default))
+     (Tcons tuint Tnil) tint cc_default)) ::
+ (___builtin_ctzl,
+   Gfun(External (EF_builtin "__builtin_ctzl"
+                   (mksignature (AST.Tint :: nil) (Some AST.Tint) cc_default))
+     (Tcons tuint Tnil) tint cc_default)) ::
+ (___builtin_ctzll,
+   Gfun(External (EF_builtin "__builtin_ctzll"
+                   (mksignature (AST.Tlong :: nil) (Some AST.Tint)
+                     cc_default)) (Tcons tulong Tnil) tint cc_default)) ::
+ (___builtin_fmax,
+   Gfun(External (EF_builtin "__builtin_fmax"
+                   (mksignature (AST.Tfloat :: AST.Tfloat :: nil)
+                     (Some AST.Tfloat) cc_default))
+     (Tcons tdouble (Tcons tdouble Tnil)) tdouble cc_default)) ::
+ (___builtin_fmin,
+   Gfun(External (EF_builtin "__builtin_fmin"
+                   (mksignature (AST.Tfloat :: AST.Tfloat :: nil)
+                     (Some AST.Tfloat) cc_default))
+     (Tcons tdouble (Tcons tdouble Tnil)) tdouble cc_default)) ::
+ (___builtin_fmadd,
+   Gfun(External (EF_builtin "__builtin_fmadd"
+                   (mksignature
+                     (AST.Tfloat :: AST.Tfloat :: AST.Tfloat :: nil)
+                     (Some AST.Tfloat) cc_default))
+     (Tcons tdouble (Tcons tdouble (Tcons tdouble Tnil))) tdouble
+     cc_default)) ::
+ (___builtin_fmsub,
+   Gfun(External (EF_builtin "__builtin_fmsub"
+                   (mksignature
+                     (AST.Tfloat :: AST.Tfloat :: AST.Tfloat :: nil)
+                     (Some AST.Tfloat) cc_default))
+     (Tcons tdouble (Tcons tdouble (Tcons tdouble Tnil))) tdouble
+     cc_default)) ::
+ (___builtin_fnmadd,
+   Gfun(External (EF_builtin "__builtin_fnmadd"
+                   (mksignature
+                     (AST.Tfloat :: AST.Tfloat :: AST.Tfloat :: nil)
+                     (Some AST.Tfloat) cc_default))
+     (Tcons tdouble (Tcons tdouble (Tcons tdouble Tnil))) tdouble
+     cc_default)) ::
+ (___builtin_fnmsub,
+   Gfun(External (EF_builtin "__builtin_fnmsub"
+                   (mksignature
+                     (AST.Tfloat :: AST.Tfloat :: AST.Tfloat :: nil)
+                     (Some AST.Tfloat) cc_default))
+     (Tcons tdouble (Tcons tdouble (Tcons tdouble Tnil))) tdouble
+     cc_default)) ::
+ (___builtin_read16_reversed,
+   Gfun(External (EF_builtin "__builtin_read16_reversed"
+                   (mksignature (AST.Tint :: nil) (Some AST.Tint) cc_default))
+     (Tcons (tptr tushort) Tnil) tushort cc_default)) ::
+ (___builtin_read32_reversed,
+   Gfun(External (EF_builtin "__builtin_read32_reversed"
+                   (mksignature (AST.Tint :: nil) (Some AST.Tint) cc_default))
+     (Tcons (tptr tuint) Tnil) tuint cc_default)) ::
+ (___builtin_write16_reversed,
+   Gfun(External (EF_builtin "__builtin_write16_reversed"
+                   (mksignature (AST.Tint :: AST.Tint :: nil) None
+                     cc_default)) (Tcons (tptr tushort) (Tcons tushort Tnil))
+     tvoid cc_default)) ::
+ (___builtin_write32_reversed,
+   Gfun(External (EF_builtin "__builtin_write32_reversed"
+                   (mksignature (AST.Tint :: AST.Tint :: nil) None
+                     cc_default)) (Tcons (tptr tuint) (Tcons tuint Tnil))
+     tvoid cc_default)) ::
+ (___builtin_nop,
+   Gfun(External (EF_builtin "__builtin_nop"
+                   (mksignature nil None cc_default)) Tnil tvoid cc_default)) ::
+ (___builtin_debug,
+   Gfun(External (EF_external "__builtin_debug"
+                   (mksignature (AST.Tint :: nil) None
+                     {|cc_vararg:=true; cc_unproto:=false; cc_structret:=false|}))
+     (Tcons tint Tnil) tvoid
+     {|cc_vararg:=true; cc_unproto:=false; cc_structret:=false|})) ::
+ (_malloc,
+   Gfun(External EF_malloc (Tcons tuint Tnil) (tptr tvoid) cc_default)) ::
+ (_calloc,
+   Gfun(External (EF_external "calloc"
+                   (mksignature (AST.Tint :: AST.Tint :: nil) (Some AST.Tint)
+                     cc_default)) (Tcons tuint (Tcons tuint Tnil))
+     (tptr tvoid) cc_default)) ::
+ (_free, Gfun(External EF_free (Tcons (tptr tvoid) Tnil) tvoid cc_default)) ::
+ (_memset,
+   Gfun(External (EF_external "memset"
+                   (mksignature (AST.Tint :: AST.Tint :: AST.Tint :: nil)
+                     (Some AST.Tint) cc_default))
+     (Tcons (tptr tvoid) (Tcons tint (Tcons tuint Tnil))) (tptr tvoid)
+     cc_default)) ::
+ (_ber_check_tags,
+   Gfun(External (EF_external "ber_check_tags"
+                   (mksignature
+                     (AST.Tint :: AST.Tint :: AST.Tint :: AST.Tint ::
+                      AST.Tint :: AST.Tint :: AST.Tint :: AST.Tint ::
+                      AST.Tint :: AST.Tint :: nil) None
+                     {|cc_vararg:=false; cc_unproto:=false; cc_structret:=true|}))
+     (Tcons (tptr (Tstruct _asn_dec_rval_s noattr))
+       (Tcons (tptr (Tstruct _asn_codec_ctx_s noattr))
+         (Tcons (tptr (Tstruct _asn_TYPE_descriptor_s noattr))
+           (Tcons (tptr (Tstruct _asn_struct_ctx_s noattr))
+             (Tcons (tptr tvoid)
+               (Tcons tuint
+                 (Tcons tint
+                   (Tcons tint (Tcons (tptr tint) (Tcons (tptr tint) Tnil))))))))))
+     tvoid {|cc_vararg:=false; cc_unproto:=false; cc_structret:=true|})) ::
+ (_der_write_tags,
+   Gfun(External (EF_external "der_write_tags"
+                   (mksignature
+                     (AST.Tint :: AST.Tint :: AST.Tint :: AST.Tint ::
+                      AST.Tint :: AST.Tint :: AST.Tint :: nil)
+                     (Some AST.Tint) cc_default))
+     (Tcons (tptr (Tstruct _asn_TYPE_descriptor_s noattr))
+       (Tcons tuint
+         (Tcons tint
+           (Tcons tint
+             (Tcons tuint
+               (Tcons
+                 (tptr (Tfunction
+                         (Tcons (tptr tvoid)
+                           (Tcons tuint (Tcons (tptr tvoid) Tnil))) tint
+                         cc_default)) (Tcons (tptr tvoid) Tnil))))))) tint
+     cc_default)) ::
+ (_xer_check_tag,
+   Gfun(External (EF_external "xer_check_tag"
+                   (mksignature (AST.Tint :: AST.Tint :: AST.Tint :: nil)
+                     (Some AST.Tint) cc_default))
+     (Tcons (tptr tvoid) (Tcons tint (Tcons (tptr tschar) Tnil))) tint
+     cc_default)) ::
+ (_asn_get_few_bits,
+   Gfun(External (EF_external "asn_get_few_bits"
+                   (mksignature (AST.Tint :: AST.Tint :: nil) (Some AST.Tint)
+                     cc_default))
+     (Tcons (tptr (Tstruct _asn_bit_data_s noattr)) (Tcons tint Tnil)) tint
+     cc_default)) ::
+ (_asn_put_few_bits,
+   Gfun(External (EF_external "asn_put_few_bits"
+                   (mksignature (AST.Tint :: AST.Tint :: AST.Tint :: nil)
+                     (Some AST.Tint) cc_default))
+     (Tcons (tptr (Tstruct _asn_bit_outp_s noattr))
+       (Tcons tuint (Tcons tint Tnil))) tint cc_default)) ::
+ (_asn_generic_no_constraint,
+   Gfun(External (EF_external "asn_generic_no_constraint"
+                   (mksignature
+                     (AST.Tint :: AST.Tint :: AST.Tint :: AST.Tint :: nil)
+                     (Some AST.Tint) cc_default))
+     (Tcons (tptr (Tstruct _asn_TYPE_descriptor_s noattr))
+       (Tcons (tptr tvoid)
+         (Tcons
+           (tptr (Tfunction
+                   (Tcons (tptr tvoid)
+                     (Tcons (tptr (Tstruct _asn_TYPE_descriptor_s noattr))
+                       (Tcons (tptr tvoid) (Tcons (tptr tschar) Tnil))))
+                   tvoid
+                   {|cc_vararg:=true; cc_unproto:=false; cc_structret:=false|}))
+           (Tcons (tptr tvoid) Tnil)))) tint cc_default)) ::
+ (_asn_generic_unknown_constraint,
+   Gfun(External (EF_external "asn_generic_unknown_constraint"
+                   (mksignature
+                     (AST.Tint :: AST.Tint :: AST.Tint :: AST.Tint :: nil)
+                     (Some AST.Tint) cc_default))
+     (Tcons (tptr (Tstruct _asn_TYPE_descriptor_s noattr))
+       (Tcons (tptr tvoid)
+         (Tcons
+           (tptr (Tfunction
+                   (Tcons (tptr tvoid)
+                     (Tcons (tptr (Tstruct _asn_TYPE_descriptor_s noattr))
+                       (Tcons (tptr tvoid) (Tcons (tptr tschar) Tnil))))
+                   tvoid
+                   {|cc_vararg:=true; cc_unproto:=false; cc_structret:=false|}))
+           (Tcons (tptr tvoid) Tnil)))) tint cc_default)) ::
+ (_asn_random_between,
+   Gfun(External (EF_external "asn_random_between"
+                   (mksignature (AST.Tlong :: AST.Tlong :: nil)
+                     (Some AST.Tlong) cc_default))
+     (Tcons tlong (Tcons tlong Tnil)) tlong cc_default)) ::
+ (_oer_decode_primitive,
+   Gfun(External (EF_external "oer_decode_primitive"
+                   (mksignature
+                     (AST.Tint :: AST.Tint :: AST.Tint :: AST.Tint ::
+                      AST.Tint :: AST.Tint :: AST.Tint :: nil) None
+                     {|cc_vararg:=false; cc_unproto:=false; cc_structret:=true|}))
+     (Tcons (tptr (Tstruct _asn_dec_rval_s noattr))
+       (Tcons (tptr (Tstruct _asn_codec_ctx_s noattr))
+         (Tcons (tptr (Tstruct _asn_TYPE_descriptor_s noattr))
+           (Tcons (tptr (Tstruct _asn_oer_constraints_s noattr))
+             (Tcons (tptr (tptr tvoid))
+               (Tcons (tptr tvoid) (Tcons tuint Tnil))))))) tvoid
+     {|cc_vararg:=false; cc_unproto:=false; cc_structret:=true|})) ::
+ (_oer_encode_primitive,
+   Gfun(External (EF_external "oer_encode_primitive"
+                   (mksignature
+                     (AST.Tint :: AST.Tint :: AST.Tint :: AST.Tint ::
+                      AST.Tint :: AST.Tint :: nil) None
+                     {|cc_vararg:=false; cc_unproto:=false; cc_structret:=true|}))
+     (Tcons (tptr (Tstruct _asn_enc_rval_s noattr))
+       (Tcons (tptr (Tstruct _asn_TYPE_descriptor_s noattr))
+         (Tcons (tptr (Tstruct _asn_oer_constraints_s noattr))
+           (Tcons (tptr tvoid)
+             (Tcons
+               (tptr (Tfunction
+                       (Tcons (tptr tvoid)
+                         (Tcons tuint (Tcons (tptr tvoid) Tnil))) tint
+                       cc_default)) (Tcons (tptr tvoid) Tnil)))))) tvoid
+     {|cc_vararg:=false; cc_unproto:=false; cc_structret:=true|})) ::
+ (_asn_TYPE_outmost_tag,
+   Gfun(External (EF_external "asn_TYPE_outmost_tag"
+                   (mksignature
+                     (AST.Tint :: AST.Tint :: AST.Tint :: AST.Tint :: nil)
+                     (Some AST.Tint) cc_default))
+     (Tcons (tptr (Tstruct _asn_TYPE_descriptor_s noattr))
+       (Tcons (tptr tvoid) (Tcons tint (Tcons tuint Tnil)))) tuint
+     cc_default)) ::
+ (_ASN__PRIMITIVE_TYPE_free,
+   Gfun(External (EF_external "ASN__PRIMITIVE_TYPE_free"
+                   (mksignature (AST.Tint :: AST.Tint :: AST.Tint :: nil)
+                     None cc_default))
+     (Tcons (tptr (Tstruct _asn_TYPE_descriptor_s noattr))
+       (Tcons (tptr tvoid) (Tcons tint Tnil))) tvoid cc_default)) ::
+ (_ber_decode_primitive,
+   Gfun(External (EF_external "ber_decode_primitive"
+                   (mksignature
+                     (AST.Tint :: AST.Tint :: AST.Tint :: AST.Tint ::
+                      AST.Tint :: AST.Tint :: AST.Tint :: nil) None
+                     {|cc_vararg:=false; cc_unproto:=false; cc_structret:=true|}))
+     (Tcons (tptr (Tstruct _asn_dec_rval_s noattr))
+       (Tcons (tptr (Tstruct _asn_codec_ctx_s noattr))
+         (Tcons (tptr (Tstruct _asn_TYPE_descriptor_s noattr))
+           (Tcons (tptr (tptr tvoid))
+             (Tcons (tptr tvoid) (Tcons tuint (Tcons tint Tnil))))))) tvoid
+     {|cc_vararg:=false; cc_unproto:=false; cc_structret:=true|})) ::
+ (_der_encode_primitive,
+   Gfun(External (EF_external "der_encode_primitive"
+                   (mksignature
+                     (AST.Tint :: AST.Tint :: AST.Tint :: AST.Tint ::
+                      AST.Tint :: AST.Tint :: AST.Tint :: nil) None
+                     {|cc_vararg:=false; cc_unproto:=false; cc_structret:=true|}))
+     (Tcons (tptr (Tstruct _asn_enc_rval_s noattr))
+       (Tcons (tptr (Tstruct _asn_TYPE_descriptor_s noattr))
+         (Tcons (tptr tvoid)
+           (Tcons tint
+             (Tcons tuint
+               (Tcons
+                 (tptr (Tfunction
+                         (Tcons (tptr tvoid)
+                           (Tcons tuint (Tcons (tptr tvoid) Tnil))) tint
+                         cc_default)) (Tcons (tptr tvoid) Tnil))))))) tvoid
+     {|cc_vararg:=false; cc_unproto:=false; cc_structret:=true|})) ::
+ (_xer_decode_primitive,
+   Gfun(External (EF_external "xer_decode_primitive"
+                   (mksignature
+                     (AST.Tint :: AST.Tint :: AST.Tint :: AST.Tint ::
+                      AST.Tint :: AST.Tint :: AST.Tint :: AST.Tint ::
+                      AST.Tint :: nil) None
+                     {|cc_vararg:=false; cc_unproto:=false; cc_structret:=true|}))
+     (Tcons (tptr (Tstruct _asn_dec_rval_s noattr))
+       (Tcons (tptr (Tstruct _asn_codec_ctx_s noattr))
+         (Tcons (tptr (Tstruct _asn_TYPE_descriptor_s noattr))
+           (Tcons (tptr (tptr tvoid))
+             (Tcons tuint
+               (Tcons (tptr tschar)
+                 (Tcons (tptr tvoid)
+                   (Tcons tuint
+                     (Tcons
+                       (tptr (Tfunction
+                               (Tcons
+                                 (tptr (Tstruct _asn_TYPE_descriptor_s noattr))
+                                 (Tcons (tptr tvoid)
+                                   (Tcons (tptr tvoid) (Tcons tuint Tnil))))
+                               tint cc_default)) Tnil))))))))) tvoid
+     {|cc_vararg:=false; cc_unproto:=false; cc_structret:=true|})) ::
+ (_asn_DEF_BOOLEAN_tags, Gvar v_asn_DEF_BOOLEAN_tags) ::
+ (_asn_OP_BOOLEAN, Gvar v_asn_OP_BOOLEAN) ::
+ (_asn_DEF_BOOLEAN, Gvar v_asn_DEF_BOOLEAN) ::
+ (_BOOLEAN_decode_ber, Gfun(Internal f_BOOLEAN_decode_ber)) ::
+ (_BOOLEAN_encode_der, Gfun(Internal f_BOOLEAN_encode_der)) ::
+ (_BOOLEAN__xer_body_decode, Gfun(Internal f_BOOLEAN__xer_body_decode)) ::
+ (_BOOLEAN_decode_xer, Gfun(Internal f_BOOLEAN_decode_xer)) ::
+ (_BOOLEAN_encode_xer, Gfun(Internal f_BOOLEAN_encode_xer)) ::
+ (_BOOLEAN_print, Gfun(Internal f_BOOLEAN_print)) ::
+ (_BOOLEAN_free, Gfun(Internal f_BOOLEAN_free)) ::
+ (_BOOLEAN_decode_uper, Gfun(Internal f_BOOLEAN_decode_uper)) ::
+ (_BOOLEAN_encode_uper, Gfun(Internal f_BOOLEAN_encode_uper)) ::
+ (_BOOLEAN_encode_oer, Gfun(Internal f_BOOLEAN_encode_oer)) ::
+ (_BOOLEAN_decode_oer, Gfun(Internal f_BOOLEAN_decode_oer)) ::
+ (_BOOLEAN_compare, Gfun(Internal f_BOOLEAN_compare)) ::
+ (_BOOLEAN_random_fill, Gfun(Internal f_BOOLEAN_random_fill)) :: nil).
+
+Definition public_idents : list ident :=
+(_BOOLEAN_random_fill :: _BOOLEAN_compare :: _BOOLEAN_decode_oer ::
+ _BOOLEAN_encode_oer :: _BOOLEAN_encode_uper :: _BOOLEAN_decode_uper ::
+ _BOOLEAN_free :: _BOOLEAN_print :: _BOOLEAN_encode_xer ::
+ _BOOLEAN_decode_xer :: _BOOLEAN_encode_der :: _BOOLEAN_decode_ber ::
+ _asn_DEF_BOOLEAN :: _asn_OP_BOOLEAN :: _xer_decode_primitive ::
+ _der_encode_primitive :: _ber_decode_primitive ::
+ _ASN__PRIMITIVE_TYPE_free :: _asn_TYPE_outmost_tag ::
+ _oer_encode_primitive :: _oer_decode_primitive :: _asn_random_between ::
+ _asn_generic_unknown_constraint :: _asn_generic_no_constraint ::
+ _asn_put_few_bits :: _asn_get_few_bits :: _xer_check_tag ::
+ _der_write_tags :: _ber_check_tags :: _memset :: _free :: _calloc ::
+ _malloc :: ___builtin_debug :: ___builtin_nop ::
+ ___builtin_write32_reversed :: ___builtin_write16_reversed ::
+ ___builtin_read32_reversed :: ___builtin_read16_reversed ::
+ ___builtin_fnmsub :: ___builtin_fnmadd :: ___builtin_fmsub ::
+ ___builtin_fmadd :: ___builtin_fmin :: ___builtin_fmax ::
+ ___builtin_ctzll :: ___builtin_ctzl :: ___builtin_ctz :: ___builtin_clzll ::
+ ___builtin_clzl :: ___builtin_clz :: ___builtin_bswap64 ::
+ ___compcert_i64_umulh :: ___compcert_i64_smulh :: ___compcert_i64_sar ::
+ ___compcert_i64_shr :: ___compcert_i64_shl :: ___compcert_i64_umod ::
+ ___compcert_i64_smod :: ___compcert_i64_udiv :: ___compcert_i64_sdiv ::
+ ___compcert_i64_utof :: ___compcert_i64_stof :: ___compcert_i64_utod ::
+ ___compcert_i64_stod :: ___compcert_i64_dtou :: ___compcert_i64_dtos ::
+ ___compcert_va_composite :: ___compcert_va_float64 ::
+ ___compcert_va_int64 :: ___compcert_va_int32 :: ___builtin_va_end ::
+ ___builtin_va_copy :: ___builtin_va_arg :: ___builtin_va_start ::
+ ___builtin_membar :: ___builtin_annot_intval :: ___builtin_annot ::
+ ___builtin_memcpy_aligned :: ___builtin_fsqrt :: ___builtin_fabs ::
+ ___builtin_bswap16 :: ___builtin_bswap32 :: ___builtin_bswap ::
+ ___builtin_ais_annot :: nil).
+
+Definition prog : Clight.program := 
+  mkprogram composites global_definitions public_idents _main Logic.I.
+
+
