asn_strtoimax_lim.v
@@ -181,6 +181,8 @@ Definition _t'4 : ident := 163%positive.
 Definition _t'5 : ident := 164%positive.
 Definition _t'6 : ident := 165%positive.
 
+Print LScons.
+
 Definition f_asn_strtoimax_lim := {|
   fn_return := tint;
   fn_callconv := cc_default;
