asn_strtoimax_lim_spec.v
@@ -1,9 +1,91 @@
-(*
- * Parse the number in the given string until the given *end position,
- * returning the position after the last parsed character back using the
- * same (*end) pointer.
- * WARNING: This behavior is different from the standard strtol/strtoimax(3).
- *)
+From Coq Require Import String List ZArith Psatz.
+From compcert Require Import Coqlib Integers Floats AST Ctypes Cop Clight Clightdefs Memory Values ClightBigstep Events Maps.
+Local Open Scope Z_scope.
+
+(* Functional specification of INTEGER.asn_strtoimax_lim
+ 
+ Parse the number in the given string until the given end position,
+  returning the position after the last parsed character back using the
+  same (end) pointer. WARNING: This behavior is different from the standard strtol/strtoimax(3). *)
+
+(* Output type of asn_strtoimax_lim *)
+
+Inductive asn_strtox_result_e :=
+  | ASN_STRTOX_ERROR_RANGE (* Input outside of supported numeric range *)
+  | ASN_STRTOX_ERROR_INVAL (* Invalid data encountered (e.g., "+-") *)
+  | ASN_STRTOX_EXPECT_MORE (* More data expected (e.g. "+") *)
+  | ASN_STRTOX_EXTRA_DATA (* Conversion succeded, but the string has extra stuff *)
+  | ASN_STRTOX_OK. (* Conversion succeded, number ends at (end) *) 
+
+Definition asn_strtox_result_e_to_int (s : asn_strtox_result_e) : int :=
+  match s with
+    | ASN_STRTOX_ERROR_RANGE => Int.repr (-1)  
+    | ASN_STRTOX_ERROR_INVAL => Int.repr (-3)
+    | ASN_STRTOX_EXPECT_MORE => Int.repr (-2)
+    | ASN_STRTOX_EXTRA_DATA => Int.repr 1 
+    | ASN_STRTOX_OK => Int.repr 0
+  end.
+
+Definition addr : Type := (block*ptrofs).
+
+(* Predicate stating that there is a C string of length n at address a1 
+Inductive Cstring (m : mem) (b : block) (ofs : ptrofs) : nat -> Prop :=
+| EmptyString: Mem.loadv Mint8signed m (Vptr b ofs) = Some (Vint Int.zero) -> Cstring m b ofs O
+| SuccString: forall n c, Mem.loadv Mint8signed m (Vptr b ofs)  = Some (Vint c) ->
+                        c <> Int.zero ->
+                        Cstring m b (Ptrofs.add ofs Ptrofs.one) n ->
+                        Cstring m b ofs (S n). *)
+  
+(* Formalize intmax_t and uintmax_t ??? Maybe use module types? *)
+
+(* /* Largest integral types.  */
+#if __WORDSIZE == 64
+typedef long int		intmax_t;
+typedef unsigned long int	uintmax_t;
+#else
+__extension__
+typedef long long int		intmax_t;
+__extension__
+typedef unsigned long long int	uintmax_t;
+#endif 
+*)
+
+Inductive intsize : Type :=
+  | I8: intsize
+  | I32: intsize
+  | I64 : intsize.
+
+Definition intmax_t (s : intsize) := match s with | I64 => Int64.int | I32 => Int.int | I8 => Byte.int end.
+
+Check Val.cmpu_bool.
+
+Variable valid_ptr: block -> Z -> bool.
+
+Definition asn_strtoimax_lim_spec_64 (m : Mem.mem) (b_str : block) (ofs_str : ptrofs)
+           (b_end : block) (ofs_end : ptrofs) : option (Int.int*block*ptrofs) :=
+  let ASN1_INTMAX_MAX := Int64.shru (Int64.not Int64.zero) Int64.one in
+        match  Val.cmpu_bool valid_ptr Cge (Vptr b_str ofs_str) (Vptr b_end ofs_str) with
+        | Some true => Some (asn_strtox_result_e_to_int ASN_STRTOX_ERROR_INVAL, b_end, ofs_end)            | _ => None
+        end.
+
+Definition asn_strtoimax_lim_spec_INT_TYPE (s : intsize) (m : Mem.mem) (pstr : addr) (pend : addr) : option (Int.int*addr) :=
+  match s with
+  | I64 => asn_strtoimax_lim_spec_64 m pstr pend
+  | _ =>  Some (Int.zero, pend)
+  end.
+  
+  
+Fact shift_pow2_div :  (Int64.shru (Int64.not Int64.zero) Int64.one) = Int64.repr (Int64.max_unsigned / 2).
+  replace (Int64.not Int64.zero) with (Int64.repr Int64.max_unsigned) by (auto with ints).
+  unfold Int64.shru.
+  f_equal.
+  Qed.
+  
+  
+  
+
+
+
 
 (* STRTOIMAX(3)               Linux Programmer's Manual              STRTOIMAX(3)
 
