README.md
@@ -1,7 +1,7 @@
 
-File *REAL.v* contains output of clightgen on REAL.c. Options ```-fstruct-passing -flongdouble``` are needed due to the features unsupported by compcert: functions returning a struct or union and long double:
+File *BOOLEAN.v* contains output of clightgen on BOOLEAN.c of asn1c. Options ```-fstruct-passing -flongdouble``` are needed due to the features unsupported by compcert: functions returning a struct or union and long double:
 
-```./clightgen -normalize -I ~/asn1c/skeletons/ -fstruct-passing -flongdouble ~/asn1c/skeletons/REAL.c -o REAL.v ```
+```./clightgen -normalize -I ~/asn1c/skeletons/ -fstruct-passing -flongdouble ~/asn1c/skeletons/BOOLEAN.c -o BOOLEAN.v ```
 
 
 To build clightgen go to compcert folder 
